Changes:  - Now computations cannot have silent labels, as it is kind of the point of the weak bisimulations that the ordering of computations is preserved.  - The above change propagated through  - Full fork commutativity proof in the sense of providing a relation R such that for all fork expressions the original and the swapped are in relation and R obeys the weak bisimilarity. (This is quite a big change, just shy of 4000 lines.)

forkProofs.v
@@ -3,11 +3,16 @@ Require Import Bool.
 Require Import List.
 Require Import Classical_Prop.
 
+
 Load mconbaseMonProofs.
 
-Check 0.
+Load LibTactics.
 
-Definition swapbodyll : expr :=  E_apply ( E_constant CONST_ret )  
+
+
+
+
+Definition swapbodyll : expr := E_apply ( E_constant CONST_ret )  
                                    ( E_taggingleft 
                                      ( E_taggingleft
                                         (E_apply 
@@ -19,13 +24,8 @@ Definition swapbodyll : expr :=  E_apply ( E_constant CONST_ret )
                                      )
                                    ).
 
-Definition swapbodyl : expr := E_case (E_ident (1)) 
-                    (3) ( 
-                          swapbodyll
-                        ) 
-                    (4) (
-                           E_apply ( E_constant CONST_ret )  
-                                   ( E_taggingleft 
+Definition swapbodylr : expr :=   E_apply ( E_constant CONST_ret )  
+                                   (
                                      ( E_taggingright
                                         (E_apply 
                                           ( E_apply (E_constant CONST_pair)  
@@ -34,43 +34,29 @@ Definition swapbodyl : expr := E_case (E_ident (1))
                                           (E_apply (E_constant CONST_proj1) (E_ident (4)))  
                                         )
                                      )
-                                   )
+                                   ).
+
+
+Definition swapbodyl : expr := E_case (E_ident (1)) 
+                    (3) ( 
+                          swapbodyll
+                        ) 
+                    (4) (
+                          swapbodylr
 
                         ).
 
-Definition swapbodyrr : expr := E_apply ( E_constant CONST_ret )  
-                                   ( E_taggingright 
+Definition swapbodyr : expr :=E_apply ( E_constant CONST_ret )  
+                                   (E_taggingleft  
                                      ( E_taggingright
                                         (E_apply 
                                           ( E_apply (E_constant CONST_pair)  
-                                                    (E_apply (E_constant CONST_proj2) (E_ident (5))) 
+                                                    (E_apply (E_constant CONST_proj2) (E_ident (2))) 
                                           ) 
-                                          (E_apply (E_constant CONST_proj1) (E_ident (5)))  
+                                          (E_apply (E_constant CONST_proj1) (E_ident (2)))  
                                         )
                                      )
-                                   ).
-
-Definition swapbodyrl : expr :=   E_apply ( E_constant CONST_ret )  
-                                   ( E_taggingright 
-                                     ( E_taggingleft
-                                        (E_apply 
-                                          ( E_apply (E_constant CONST_pair)  
-                                                    (E_apply (E_constant CONST_proj2) (E_ident (6))) 
-                                          ) 
-                                          (E_apply (E_constant CONST_proj1) (E_ident (6)))  
-                                        )
-                                     )
-                                   ).
-
-Definition swapbodyr : expr :=  E_case (E_ident (2)) 
-                    (5) ( 
-                           swapbodyrr
-                        ) 
-                    (6) (
-                         
-                           swapbodyrl
-
-                        ).
+                                    ).
 
 Definition swapbody : expr := E_case (E_ident (0)) 
            (1) ( 
@@ -289,28 +275,25 @@ rewrite <- H3 in H; simpl in H; auto.
  rewrite <- H7 in H; simpl in H; auto; intuition.
  rewrite <- H6 in H; simpl in H; auto; intuition.
  rewrite <- H7 in H; simpl in H; auto; intuition.
- rewrite <- H7 in H; simpl in H; auto; intuition.
- rewrite <- H7 in H; simpl in H; auto; intuition.
- rewrite <- H7 in H; simpl in H; auto; intuition.
- rewrite <- H7 in H; simpl in H; auto; intuition.
- rewrite <- H7 in H; simpl in H; auto; intuition.
- contradiction.
- inversion H0; intuition.
- cut (tauStep e' e''0).
- intros.
- apply H16 in H15.
- rewrite H15; reflexivity.
- apply tStep with (s:=s).
- trivial.
- contradiction.
- contradiction.
- contradiction.
- rewrite <- H6 in H; simpl in H; intuition.
- rewrite <- H6 in H2; rewrite <- H6 in H1; rewrite <- H6 in H0.
- rewrite <- H10 in H2.
- rewrite <- H10 in H7.
+ substs.
  intuition.
- rewrite <- H6 in H; simpl in H; rewrite <- H10 in H9; intuition.
+ substs; simpl in H; auto; intuition.
+ inverts H0.
+ intuition.
+ f_equal.
+ apply H5. 
+ apply tStep with (s:=s); trivial.
+ substs.
+ contradiction.
+ substs.
+ contradiction.
+ substs.
+ contradiction.
+ substs.
+ simpl in H.
+ intuition.
+ substs.
+ simpl in H; intuition.
 Qed.
 
 Lemma simpTau : forall(e e' : expr) (s: select),  
@@ -419,31 +402,215 @@ rewrite <- H3 in H0; simpl in H0; intuition.
  rewrite <- H6 in H0; simpl in H0; auto; intuition.
  rewrite <- H6 in H0; simpl in H0; auto; intuition.
  rewrite <- H6 in H0; simpl in H0; auto; intuition.
- rewrite <- H6 in H0; simpl in H0; auto; intuition.
- rewrite <- H7 in H0; simpl in H0; auto; intuition.
- rewrite <- H7 in H0; simpl in H0; auto; intuition.
- rewrite <- H7 in H0; simpl in H0; auto; intuition.
- rewrite <- H7 in H0; simpl in H0; auto; intuition.
- rewrite <- H7 in H0; simpl in H0; auto; intuition.
- rewrite <- H7 in H0; simpl in H0; auto; intuition.
- rewrite <- H6 in H0; simpl in H0; auto; intuition.
- apply red_not_value in H11.
- contradiction.
- cut (tauStep e e'1).
- intros.
+ rewrite <- H6 in H0; simpl in H0; auto; intuition. 
+ substs.
+ simpl in H0; intuition.
+ substs.
+ apply red_not_value in H11; contradiction.
+ substs.
+ f_equal.
  inversion H1.
- intuition.
- apply H19 in H13.
- rewrite H13; reflexivity.
- 
- eauto.
- rewrite <- H6 in H0; simpl in H0.
- contradiction.
- rewrite <- H6 in H0; simpl in H0;
- contradiction.
- rewrite <- H6 in H0; simpl in H0; intuition.
- rewrite <- H6 in H0; simpl in H0; intuition.
+ substs; intuition; substs.
+ apply H7.
+ apply simpTau with (s:=s).
+ trivial.
+ substs.
+ simpl in H0; intuition.
+ substs.
+ simpl in H0; intuition.
+ substs.
+ simpl in H0; intuition.
+ substs.
+ simpl in H0; intuition.
 Qed.
+
+
+Lemma swapf_right : forall (v v' : expr), 
+           is_value_of_expr v ->
+           is_value_of_expr v' ->
+           totalTauRed ( E_apply (swapf) (E_taggingright (( E_pair v v' )) ) ) (E_live_expr(LM_expr(E_taggingleft(E_taggingright ( ( E_pair v' v )) )))).
+Proof.
+ intros.
+ apply S_star with (y:=(subst_expr (E_taggingright ( ( E_pair v v' ))) 0 swapbody )).
+ apply JO_red_app_td.
+ simpl.
+ auto.
+ simpl.
+ apply S_star with (y:=(subst_expr   ( ( E_pair v v' ))   2   swapbodyr )).
+ apply JO_red_evalcaseinr_td.
+ simpl; auto.
+ apply S_star with (y:=E_apply ( E_constant CONST_ret )
+                                    ( E_taggingleft 
+                                     ( E_taggingright
+                                        (E_apply 
+                                          ( E_apply (E_constant CONST_pair)  
+                                                    (E_apply (E_constant CONST_proj2) ( E_pair v v' )) 
+                                          ) 
+                                          (v)  
+                                        )
+                                     ))).
+ simpl.
+ apply JO_red_context_app1_td.
+ simpl.
+ intuition.
+ apply JO_red_evalinl_td.
+ simpl; auto.
+  apply JO_red_evalinr_td.
+ simpl; auto.
+ apply JO_red_context_app1_td.
+ simpl; auto.
+ apply JO_red_proj1_td.
+ trivial.
+ trivial.
+ apply S_star with (y:=E_apply ( E_constant CONST_ret ) 
+                                    ( E_taggingleft 
+                                     ( E_taggingright
+                                        (E_apply 
+                                          ( E_apply (E_constant CONST_pair)  
+                                                    (v') 
+                                          ) 
+                                          (v)  
+                                        )
+                                     ))).
+ apply JO_red_context_app1_td.
+ simpl; auto.
+ apply JO_red_evalinl_td.
+ simpl; auto.
+  apply JO_red_evalinr_td.
+ simpl; auto.
+ apply JO_red_context_app2_td.
+ simpl; auto.
+ simpl; auto.
+ apply JO_red_context_app1_td.
+ simpl; auto.
+ apply JO_red_proj2_td.
+ trivial.
+ trivial.
+ apply S_star with (y:=((E_apply (E_constant CONST_ret)
+     ( E_taggingleft (
+        (E_taggingright (E_pair v' v))))))).
+ apply JO_red_context_app1_td.
+ simpl; auto.
+ apply JO_red_evalinl_td.
+ simpl; auto.
+ apply JO_red_evalinr_td.
+ simpl; auto.
+ apply JO_red_inpair_td.
+ simpl; auto.
+ simpl; auto.
+ apply S_star with (y:=(E_live_expr (LM_expr (E_taggingleft (E_taggingright((E_pair v' v))))))).
+ apply JO_red_ret_td.
+ apply S_First.
+ simpl;auto.
+ apply star_refl.
+Qed.
+
+Lemma swapf_right_b : forall (v v' : expr), 
+           is_value_of_expr v ->
+           is_value_of_expr v' ->
+           totalTauRed ( (E_live_expr ( LM_expr (E_taggingright (( E_pair v v' )))) ) >>= swapf) (E_live_expr(LM_expr(E_taggingleft(E_taggingright ( ( E_pair v' v )) )))).
+Proof.
+ intros.
+ apply S_star  with (y:=(E_apply (swapf) (E_taggingright (( E_pair v v' )) ))).
+ apply JO_red_dobind_td.
+ apply S_First.
+ simpl; auto.
+ apply swapf_right.
+ assumption.
+ assumption.
+Qed.
+
+Lemma swapf_left_right : forall (v v' : expr), 
+           is_value_of_expr v ->
+           is_value_of_expr v' ->
+           totalTauRed ( E_apply (swapf) (E_taggingleft (E_taggingright ( E_pair v v' )) ) ) (E_live_expr(LM_expr( (E_taggingright ( E_pair v' v )) ))).
+Proof.
+ intros.
+ apply S_star with (y:=(subst_expr (E_taggingleft (E_taggingright ( E_pair v v' ))) 0 swapbody )).
+ apply JO_red_app_td.
+ simpl.
+ auto.
+ simpl.
+ apply S_star with (y:=(subst_expr   (E_taggingright ( E_pair v v' ))   1   swapbodyl )).
+ apply JO_red_evalcaseinl_td.
+ simpl; auto.
+ apply S_star with (y:=(subst_expr    ( E_pair v v' )   4   swapbodylr )).
+ simpl.
+ apply JO_red_evalcaseinr_td.
+ simpl; auto.
+ simpl.
+ apply S_star with (y:=E_apply ( E_constant CONST_ret )  
+                                   (  
+                                     ( E_taggingright
+                                        (E_apply 
+                                          ( E_apply (E_constant CONST_pair)  
+                                                    (E_apply (E_constant CONST_proj2) (E_pair v v' )) 
+                                          ) 
+                                          (v)  
+                                        )
+                                     )
+                                   )).
+ simpl.
+ apply JO_red_context_app1_td.
+ simpl.
+ intuition.
+ apply JO_red_evalinr_td.
+ simpl; auto.
+ apply JO_red_context_app1_td.
+ simpl; auto.
+ apply JO_red_proj1_td.
+ trivial.
+ trivial.
+ apply S_star with (y:=(E_apply (E_constant CONST_ret)
+       (
+          (E_taggingright
+             (E_apply
+                (E_apply (E_constant CONST_pair)
+                   (v')) v))))).
+ apply JO_red_context_app1_td.
+ simpl; auto.
+  apply JO_red_evalinr_td.
+ simpl; auto.
+ apply JO_red_context_app2_td.
+ simpl; auto.
+ simpl; auto.
+ apply JO_red_context_app1_td.
+ simpl; auto.
+ apply JO_red_proj2_td.
+ trivial.
+ trivial.
+ apply S_star with (y:=((E_apply (E_constant CONST_ret)
+     (
+        (E_taggingright (E_pair v' v)))))).
+ apply JO_red_context_app1_td.
+ simpl; auto.
+ apply JO_red_evalinr_td.
+ simpl; auto.
+ apply JO_red_inpair_td.
+ simpl; auto.
+ simpl; auto.
+ apply S_star with (y:=(E_live_expr (LM_expr ((E_taggingright (E_pair v' v)))))).
+ apply JO_red_ret_td.
+ apply S_First.
+ simpl;auto.
+ apply star_refl.
+Qed.
+
+Lemma swapf_left_right_b : forall (v v' : expr), 
+           is_value_of_expr v ->
+           is_value_of_expr v' ->
+           totalTauRed (  (E_live_expr(LM_expr(E_taggingleft (E_taggingright ( E_pair v v' )) ))) >>= (swapf)) (E_live_expr(LM_expr( (E_taggingright ( E_pair v' v )) ))).
+Proof.
+ intros.
+ apply S_star  with (y:=(E_apply (swapf) ((E_taggingleft (E_taggingright (E_pair v v')) )))).
+ apply JO_red_dobind_td.
+ apply S_First.
+ simpl; auto.
+ apply swapf_left_right.
+ assumption.
+ assumption.
+Qed.
+
 
 Lemma swapf_left_left : forall (v v' : expr), 
            is_value_of_expr v ->
@@ -460,8 +627,10 @@ Proof.
  apply JO_red_evalcaseinl_td.
  simpl; auto.
  apply S_star with (y:=(subst_expr    ( E_pair v v' )   3   swapbodyll )).
+ simpl.
  apply JO_red_evalcaseinl_td.
  simpl; auto.
+ simpl.
  apply S_star with (y:=E_apply ( E_constant CONST_ret )  
                                    ( E_taggingleft 
                                      ( E_taggingleft
@@ -525,193 +694,3118 @@ Proof.
  apply star_refl.
 Qed.
 
-
-Lemma swapf_right_right : forall (v v' : expr), 
+Lemma swapf_left_left_b : forall (v v' : expr), 
            is_value_of_expr v ->
            is_value_of_expr v' ->
-           totalTauRed ( E_apply (swapf) (E_taggingright (E_taggingright ( E_pair v v' )) ) ) (E_live_expr(LM_expr(E_taggingright (E_taggingleft ( E_pair v' v )) ))).
+           totalTauRed (  (E_live_expr(LM_expr(E_taggingleft (E_taggingleft ( E_pair v v' )) ))) >>= (swapf)) (E_live_expr(LM_expr(E_taggingleft (E_taggingleft ( E_pair v' v )) ))).
 Proof.
  intros.
- apply S_star with (y:=(subst_expr (E_taggingright (E_taggingright ( E_pair v v' ))) 0 swapbody )).
- apply JO_red_app_td.
- simpl.
- auto.
- simpl.
- apply S_star with (y:=(subst_expr   (E_taggingright ( E_pair v v' ))   2   swapbodyr )).
- apply JO_red_evalcaseinr_td.
- simpl; auto.
- apply S_star with (y:=(subst_expr    ( E_pair v v' )   6   swapbodyrl )).
- simpl.
- apply JO_red_evalcaseinr_td.
- simpl; auto.
- simpl.
- apply S_star with (y:=E_apply ( E_constant CONST_ret )  
-                                   ( E_taggingright 
-                                     ( E_taggingleft
-                                        (E_apply 
-                                          ( E_apply (E_constant CONST_pair)  
-                                                    (E_apply (E_constant CONST_proj2) (E_pair v v' )) 
-                                          ) 
-                                          (v)  
-                                        )
-                                     )
-                                   )).
- simpl.
- apply JO_red_context_app1_td.
- simpl.
- intuition.
- apply JO_red_evalinr_td.
- simpl; auto.
- apply JO_red_evalinl_td.
- simpl; auto.
- apply JO_red_context_app1_td.
- simpl; auto.
- apply JO_red_proj1_td.
- trivial.
- trivial.
- apply S_star with (y:=(E_apply (E_constant CONST_ret)
-       (E_taggingright
-          (E_taggingleft
-             (E_apply
-                (E_apply (E_constant CONST_pair)
-                   (v')) v))))).
- apply JO_red_context_app1_td.
- simpl; auto.
-  apply JO_red_evalinr_td.
- simpl; auto.
- apply JO_red_evalinl_td.
- simpl; auto.
- apply JO_red_context_app2_td.
- simpl; auto.
- simpl; auto.
- apply JO_red_context_app1_td.
- simpl; auto.
- apply JO_red_proj2_td.
- trivial.
- trivial.
- apply S_star with (y:=((E_apply (E_constant CONST_ret)
-     (E_taggingright
-        (E_taggingleft (E_pair v' v)))))).
- apply JO_red_context_app1_td.
- simpl; auto.
- apply JO_red_evalinr_td.
- simpl; auto.
- apply JO_red_evalinl_td.
- simpl; auto.
- apply JO_red_inpair_td.
- simpl; auto.
- simpl; auto.
- apply S_star with (y:=(E_live_expr (LM_expr (E_taggingright (E_taggingleft (E_pair v' v)))))).
- apply JO_red_ret_td.
+ apply S_star  with (y:=(E_apply (swapf) ((E_taggingleft (E_taggingleft (E_pair v v')))))).
+ apply JO_red_dobind_td.
  apply S_First.
- simpl;auto.
+ simpl; auto.
+ apply swapf_left_left.
+ assumption.
+ assumption.
+Qed.
+
+Lemma simp_lab_r : forall (e e' : expr) (s :select) (l : label), JO_red e s (RL_labelled l) e' -> labRed l e e'.
+Proof.
+ intros.
+ apply lab_r with (e1:=e)(e2:=e')(s:=s).
+ splits.
+ apply star_refl.
+ trivial.
  apply star_refl.
 Qed.
 
+Inductive fork_tau_ce_int_s : relation expr :=
+ | fork_tau_ce_int_step : forall (e e' : expr) (l : label), tauStep e e' -> fork_tau_ce_int_s (E_apply (E_apply (E_constant CONST_fork) (E_live_expr (LM_comp l)))
+          (E_live_expr (LM_expr e))) (E_apply (E_apply (E_constant CONST_fork) (E_live_expr (LM_comp l)))
+          (E_live_expr (LM_expr e'))).
+Inductive fork_tau_ce_ext_s : relation expr :=
+ | fork_tau_ce_ext_step : forall (e e' : expr) (l : label), tauStep (E_apply (E_apply (E_constant CONST_fork) (E_live_expr (LM_comp l)))
+          (E_live_expr (LM_expr e))) e' -> fork_tau_ce_ext_s (E_apply (E_apply (E_constant CONST_fork) (E_live_expr (LM_comp l)))
+          (E_live_expr (LM_expr e))) e'.
 
-Lemma swapf_right_left : forall (v v' : expr), 
-           is_value_of_expr v ->
-           is_value_of_expr v' ->
-           totalTauRed ( E_apply (swapf) (E_taggingright (E_taggingleft ( E_pair v v' )) ) ) (E_live_expr(LM_expr(E_taggingright (E_taggingright ( E_pair v' v )) ))).
+
+
+Lemma fork_tau_behave_ce: forall (expr5 e : expr) (lab : label), tauRed (E_apply (E_apply (E_constant CONST_fork) (E_live_expr (LM_comp lab)))
+          (E_live_expr (LM_expr expr5))) e -> e = (E_apply (E_apply (E_constant CONST_fork) (E_live_expr (LM_comp lab)))
+          (E_live_expr (LM_expr expr5))) .
 Proof.
  intros.
- apply S_star with (y:=(subst_expr (E_taggingright (E_taggingleft ( E_pair v v' ))) 0 swapbody )).
- apply JO_red_app_td.
- simpl.
+ inversion H.
+ substs.
  auto.
- simpl.
- apply S_star with (y:=(subst_expr   (E_taggingleft ( E_pair v v' ))   2   swapbodyr )).
- apply JO_red_evalcaseinr_td.
- simpl; auto.
- apply S_star with (y:=(subst_expr    ( E_pair v v' )   5   swapbodyrr )).
- simpl.
- apply JO_red_evalcaseinl_td.
- simpl; auto.
- simpl.
- apply S_star with (y:=E_apply ( E_constant CONST_ret )  
-                                   ( E_taggingright 
-                                     ( E_taggingright
-                                        (E_apply 
-                                          ( E_apply (E_constant CONST_pair)  
-                                                    (E_apply (E_constant CONST_proj2) (E_pair v v' )) 
-                                          ) 
-                                          (v)  
-                                        )
-                                     )
-                                   )).
- simpl.
- apply JO_red_context_app1_td.
- simpl.
- intuition.
- apply JO_red_evalinr_td.
- simpl; auto.
- apply JO_red_evalinr_td.
- simpl; auto.
- apply JO_red_context_app1_td.
- simpl; auto.
- apply JO_red_proj1_td.
- trivial.
- trivial.
- apply S_star with (y:=(E_apply (E_constant CONST_ret)
-       (E_taggingright
-          (E_taggingright
-             (E_apply
-                (E_apply (E_constant CONST_pair)
-                   (v')) v))))).
- apply JO_red_context_app1_td.
- simpl; auto.
-  apply JO_red_evalinr_td.
- simpl; auto.
- apply JO_red_evalinr_td.
- simpl; auto.
- apply JO_red_context_app2_td.
- simpl; auto.
- simpl; auto.
- apply JO_red_context_app1_td.
- simpl; auto.
- apply JO_red_proj2_td.
- trivial.
- trivial.
- apply S_star with (y:=((E_apply (E_constant CONST_ret)
-     (E_taggingright
-        (E_taggingright (E_pair v' v)))))).
- apply JO_red_context_app1_td.
- simpl; auto.
- apply JO_red_evalinr_td.
- simpl; auto.
- apply JO_red_evalinr_td.
- simpl; auto.
- apply JO_red_inpair_td.
- simpl; auto.
- simpl; auto.
- apply S_star with (y:=(E_live_expr (LM_expr (E_taggingright (E_taggingright (E_pair v' v)))))).
- apply JO_red_ret_td.
- apply S_First.
- simpl;auto.
- apply star_refl.
+ substs.
+ inversion H0.
+ substs.
+ inversion H2.
+ apply red_not_value in H8; simpl in H8; intuition.
+ apply red_not_value in H9; simpl in H9; intuition.
 Qed.
 
-(*
-Theorem fork_comm : forall (e e': livemodes), weakbisim (E_apply (E_apply (E_constant CONST_fork) (E_live_expr (e))) (E_live_expr (e'))) (E_bind (E_apply (E_apply (E_constant CONST_fork) (E_live_expr (e'))) (E_live_expr (e))) (swapf)).
+Lemma fork_label_origin_ce: forall (expr5 e : expr) (lab l : label), labRed l (E_apply (E_apply (E_constant CONST_fork) (E_live_expr (LM_comp lab)))
+          (E_live_expr (LM_expr expr5))) e -> (l=lab).
 Proof.
  intros.
- induction e; induction e'.
- apply weakbi.
- split.
- apply weaksim_gen.
+ inversion H; intuition; substs.
+ apply fork_tau_behave_ce in H4.
+ substs.
+ inversion H0; intuition; substs.
+ apply red_not_value in H7; simpl in H7; intuition.
+ apply red_not_value in H8; simpl in H8; intuition.
+Qed.
+
+Lemma fork_tau_behave_ec: forall (expr5 e : expr) (lab : label), tauRed (E_apply (E_apply (E_constant CONST_fork) (E_live_expr (LM_expr expr5)) ) (E_live_expr (LM_comp lab))) e -> e = (E_apply (E_apply (E_constant CONST_fork) (E_live_expr (LM_expr expr5))) (E_live_expr (LM_comp lab))) .
+Proof.
+ intros.
+ inversion H.
+ substs.
+ auto.
+ substs.
+ inversion H0.
+ substs.
+ inversion H2.
+ apply red_not_value in H8; simpl in H8; intuition.
+ apply red_not_value in H9; simpl in H9; intuition.
+Qed.
+
+Lemma fork_label_origin_ec: forall (expr5 e : expr) (lab l : label), labRed l (E_apply (E_apply (E_constant CONST_fork) (E_live_expr (LM_expr expr5))) (E_live_expr (LM_comp lab))) e -> (l=lab (* \/ (exists (e' : expr), labRed l expr5 e' /\ e = (E_apply (E_apply (E_constant CONST_fork) (E_live_expr (LM_expr e'))) (E_live_expr (LM_comp lab))))*)).
+Proof.
+ intros.
+ inversion H; intuition; substs.
+ apply fork_tau_behave_ec in H4.
+ substs.
+ inversion H0; intuition; substs.
+ apply red_not_value in H7; simpl in H7; intuition.
+ apply red_not_value in H8; simpl in H8; intuition.
+Qed.
+
+Lemma fork_tau_behave_cc : forall (e : expr) (lab1 lab2 : label), tauRed (E_apply (E_apply (E_constant CONST_fork) (E_live_expr (LM_comp lab1))) (E_live_expr (LM_comp lab2))) e -> e= (E_apply (E_apply (E_constant CONST_fork) (E_live_expr (LM_comp lab1))) (E_live_expr (LM_comp lab2))).
+Proof.
+ intros.
+ inversion H.
+ reflexivity.
+ substs.
+ inversion H0.
+ substs.
+ inversion H2.
+ substs.
+  apply red_not_value in H8; simpl in H8; intuition.
+ apply red_not_value in H9; simpl in H9; intuition.
+Qed.
+
+Lemma fork_label_origin_cc: forall (e : expr) (lab1 lab2 l : label), labRed l (E_apply (E_apply (E_constant CONST_fork) (E_live_expr (LM_comp lab1))) (E_live_expr (LM_comp lab2))) e -> 
+((l=lab1 /\ e = (E_apply (E_apply (E_constant CONST_fork) (E_live_expr (LM_expr (E_constant CONST_unit)))) (E_live_expr (LM_comp lab2)))) \/ (l=lab2 /\ e =(E_apply (E_apply (E_constant CONST_fork) (E_live_expr (LM_comp lab1))) (E_live_expr (LM_expr (E_constant CONST_unit)))) )).
+Proof.
+ intros.
+ inversion H; intuition; substs.
+ inversion H4; intuition; substs.
+ inversion H0; intuition; substs.
+ left. splits. reflexivity.
+ inversion H6. reflexivity. substs. inversion H1. substs.
+ inversion H3.
+ apply red_not_value in H11; simpl in H11; intuition.
+ apply red_not_value in H12; simpl in H12; intuition.
+ right.
+ splits. reflexivity.
+ inversion H6. reflexivity. substs. inversion H1. substs.
+ inversion H3.
+ apply red_not_value in H11; simpl in H11; intuition.
+ apply red_not_value in H12; simpl in H12; intuition.
+ apply red_not_value in H8; simpl in H8; intuition.
+ apply red_not_value in H9; simpl in H9; intuition.
+ inversion H1; intuition; substs.
+ inversion H3; intuition; substs.
+ apply red_not_value in H11; simpl in H11; intuition.
+ apply red_not_value in H12; simpl in H12; intuition.
+Qed.
+
+
+Lemma fork_tau_step_behave_ee: forall (p q e : expr), tauStep (E_apply (E_apply (E_constant CONST_fork) (E_live_expr (LM_expr p)) ) (E_live_expr (LM_expr q))) e -> 
+   ((exists (p' q' : expr), tauRed p p' /\ tauRed q q' /\ e = (E_apply (E_apply (E_constant CONST_fork) (E_live_expr (LM_expr p')) ) (E_live_expr (LM_expr q')))) \/ 
+  ((exists (p' vq : expr), is_value_of_expr vq /\ tauRed p p' /\ tauRed q vq /\ e = ((E_live_expr (LM_expr  (  (E_taggingright  (E_pair  (E_live_expr (LM_expr p')) vq ) ) ) )))) \/ 
+  ((exists (vp vq : expr), is_value_of_expr vq /\ is_value_of_expr vp /\ tauRed p vp /\ tauRed q vq /\ e = ((E_live_expr (LM_expr  (E_taggingleft  (E_taggingleft  (E_pair vp  vq ) ) ) )))) \/ 
+   (exists (vp q' : expr), is_value_of_expr vp /\ tauRed p vp /\ tauRed q q' /\ e=((E_live_expr (LM_expr  (E_taggingleft  (E_taggingright  (E_pair vp (E_live_expr (LM_expr q'))  ) ) ) ))))))) .
+Proof.
+ intros.
+ inversion H.
+ substs.
+ inversion H0; intuition; substs.
+ left.
+ exists e'' q; splits.
+ apply S_star with (y:=e''); [ apply tStep with (s:=s0); assumption | apply star_refl]. apply star_refl.
+ reflexivity.
+ left.
+ exists p e''; splits.
+ apply star_refl.
+ apply S_star with (y:=e''); [  apply tStep with (s:=s0); assumption | apply star_refl ]. 
+ reflexivity.
+ right. right. right.
+ exists p q.
+ splits; [ assumption | apply star_refl | apply star_refl | reflexivity ].
+ right. left.
+ exists p q.
+ splits; [ assumption | apply star_refl | apply star_refl | reflexivity ].
+ right. right. left.
+ exists p q.
+ splits; [ assumption | assumption | apply star_refl | apply star_refl | reflexivity ].
+ apply red_not_value in H6; simpl in H6; intuition.
+ apply red_not_value in H7; simpl in H7; intuition.
+Qed.
+
+
+Definition  fork_tau_step_ee : expr -> expr -> Prop := (fun b e => (forall (p q : expr), b=(E_apply (E_apply (E_constant CONST_fork) (E_live_expr (LM_expr p)) ) (E_live_expr (LM_expr q))) -> 
+   ((exists (p' q' : expr), tauRed p p' /\ tauRed q q' /\ e = (E_apply (E_apply (E_constant CONST_fork) (E_live_expr (LM_expr p')) ) (E_live_expr (LM_expr q')))) \/ 
+  ((exists (p' vq : expr), is_value_of_expr vq /\ tauRed p p' /\ tauRed q vq /\ e = ((E_live_expr (LM_expr  (  (E_taggingright  (E_pair  (E_live_expr (LM_expr p')) vq ) ) ) )))) \/ 
+  ((exists (vp vq : expr), is_value_of_expr vq /\ is_value_of_expr vp /\ tauRed p vp /\ tauRed q vq /\ e = ((E_live_expr (LM_expr  (E_taggingleft  (E_taggingleft  (E_pair vp  vq ) ) ) )))) \/ 
+   (exists (vp q' : expr), is_value_of_expr vp /\ tauRed p vp /\ tauRed q q' /\ e=((E_live_expr (LM_expr  (E_taggingleft  (E_taggingright  (E_pair vp (E_live_expr (LM_expr q'))  ) ) ) ))))))))) .
+
+
+Lemma fork_tau_behave_ee_h: forall (b e : expr), tauRed b e -> (fork_tau_step_ee) b e.
+Proof.
+ apply star_ind.
+ intros.
+ unfolds.
+ intros.
+ substs.
+ left; exists p q; splits; [apply star_refl | apply star_refl | reflexivity].
+ intros.
+ unfolds in H1.
+ unfolds.
+ intros.
+ substs.
+ apply fork_tau_step_behave_ee in H.
+ intuition.
+ destruct H2; destruct H.
+ specialize (H1 x x0).
+ elim H; intros; elim H3; intros.
+ apply H1 in H5.
+ destruct H5.
+ left.
+ destruct H5 as [ p' H5]; destruct H5 as [ q' H5 ].
+ exists p' q'.
+ splits.
+ apply star_trans with (y:=x); [ jauto | jauto ].
+ apply star_trans with (y:=x0); [ jauto | jauto ].
+ jauto.
+ destruct H5.
+ right; left.
+ destruct H5 as [ p' H5]; destruct H5 as [ vq H5 ].
+ exists p' vq.
+ splits.
+ jauto.
+ apply star_trans with (y:=x); [ jauto | jauto ].
+ apply star_trans with (y:=x0); [ jauto | jauto ].
+ jauto.
+ destruct H5.
+ right; right.
+ destruct H5 as [ vp H5]; destruct H5 as [ vq H5 ].
+ left.
+ exists vp vq.
+ splits.
+ jauto.
+ jauto.
+ apply star_trans with (y:=x); [ jauto | jauto ].
+ apply star_trans with (y:=x0); [ jauto | jauto ].
+ jauto.
+ right; right.
+ right.
+ destruct H5 as [ vp H5]; destruct H5 as [ q' H5 ].
+ exists vp q'.
+ splits.
+ jauto.
+ jauto.
+ apply star_trans with (y:=x); [ jauto | jauto ].
+ apply star_trans with (y:=x0); [ jauto | jauto ].
+ jauto.
+ destruct H as [ x H]; destruct H as [ vy H ].
+ right; left.
+ exists x vy.
+ splits. jauto. jauto. jauto.
+ elim H; intros; clear H; elim H3; intros; clear H3; elim H4; intros; clear H4; substs.
+ inversion H0.
+ reflexivity.
+ inversion H4.
+ apply red_not_value in H8; simpl in H8; intuition.
+ right; right; left.
+ destruct H2 as [ vp H2]; destruct H2 as [ vq H2 ]; exists vp vq; splits; jauto;jauto;jauto;jauto.
+ elim H2; intros; clear H2. elim H3; intros; clear H3; elim H4; intros; clear H4; elim H5; intros; clear H5; substs.
+ inversion H0 ; [  reflexivity |  inversion H5; apply red_not_value in H9; simpl in H9; intuition].
+ right; right; right.
+ destruct H2 as [ vp H2]; destruct H2 as [ q' H2 ]; exists vp q'; splits; jauto;jauto;jauto.
+ elim H2; intros; clear H2; elim H3; intros; clear H3; elim H4; intros; clear H4; substs.
+ inversion H0; [ reflexivity | inversion H4; apply red_not_value in H8; simpl in H8; intuition ].
+Qed.
+ 
+Lemma fork_tau_behave_ee : forall (p q e : expr), tauRed (E_apply (E_apply (E_constant CONST_fork) (E_live_expr (LM_expr p)) ) (E_live_expr (LM_expr q))) e -> 
+((exists (p' q' : expr), tauRed p p' /\ tauRed q q' /\ e = (E_apply (E_apply (E_constant CONST_fork) (E_live_expr (LM_expr p')) ) (E_live_expr (LM_expr q')))) \/ 
+  ((exists (p' vq : expr), is_value_of_expr vq /\ tauRed p p' /\ tauRed q vq /\ e = ((E_live_expr (LM_expr  (  (E_taggingright  (E_pair  (E_live_expr (LM_expr p')) vq ) ) ) )))) \/ 
+  ((exists (vp vq : expr), is_value_of_expr vq /\ is_value_of_expr vp /\ tauRed p vp /\ tauRed q vq /\ e = ((E_live_expr (LM_expr  (E_taggingleft  (E_taggingleft  (E_pair vp  vq ) ) ) )))) \/ 
+   (exists (vp q' : expr), is_value_of_expr vp /\ tauRed p vp /\ tauRed q q' /\ e=((E_live_expr (LM_expr  (E_taggingleft  (E_taggingright  (E_pair vp (E_live_expr (LM_expr q'))  ) ) ) ))))))) .
+Proof.
+ intros.
+ apply fork_tau_behave_ee_h in H.
+ specialize (H p q).
+ apply H.
+ reflexivity.
+Qed.
+
+Lemma fork_label_origin_ee : forall (e' e e'' : expr) (l : label), labRed l (E_apply (E_apply (E_constant CONST_fork) (E_live_expr (LM_expr e)) ) (E_live_expr (LM_expr e'))) e'' -> 
+ ((exists (f : expr), labRed l e f /\ (
+((exists ( q' : expr), tauRed e' q' /\ e'' = (E_apply (E_apply (E_constant CONST_fork) (E_live_expr (LM_expr f)) ) (E_live_expr (LM_expr q')))) \/ 
+  ((exists ( vq : expr), is_value_of_expr vq /\ tauRed e' vq /\ e'' = ((E_live_expr (LM_expr  (  (E_taggingright  (E_pair  (E_live_expr (LM_expr f)) vq ) ) ) )))) \/ 
+  ((exists ( vq : expr), is_value_of_expr vq /\ is_value_of_expr f /\ tauRed e' vq /\ e'' = ((E_live_expr (LM_expr  (E_taggingleft  (E_taggingleft  (E_pair f  vq ) ) ) )))) \/ 
+   (exists ( q' : expr), is_value_of_expr f /\  tauRed e' q' /\ e''=((E_live_expr (LM_expr  (E_taggingleft  (E_taggingright  (E_pair f (E_live_expr (LM_expr q'))  ) ) ) )))))))
+
+)) 
+
+
+\/ 
+  (exists (f : expr), labRed l e' f /\ (
+((exists (p'  : expr), tauRed e p' /\ e'' = (E_apply (E_apply (E_constant CONST_fork) (E_live_expr (LM_expr p')) ) (E_live_expr (LM_expr f)))) \/ 
+  ((exists (p'  : expr), is_value_of_expr f /\ tauRed e p'  /\ e'' = ((E_live_expr (LM_expr  (  (E_taggingright  (E_pair  (E_live_expr (LM_expr p')) f ) ) ) )))) \/ 
+  ((exists (vp : expr), is_value_of_expr f /\ is_value_of_expr vp /\ tauRed e vp  /\ e'' = ((E_live_expr (LM_expr  (E_taggingleft  (E_taggingleft  (E_pair vp  f ) ) ) )))) \/ 
+   (exists (vp : expr), is_value_of_expr vp /\ tauRed e vp  /\ e''=((E_live_expr (LM_expr  (E_taggingleft  (E_taggingright  (E_pair vp (E_live_expr (LM_expr f))  ) ) ) ))))))) 
+
+))).
+Proof.
+ intros.
+ inversion H; substs.
+ elim H0; intros; substs; clear H0.
+ apply fork_tau_behave_ee in H1.
+ destruct H1.
+ destruct H0; destruct H0.
+ elim H0; intros; clear H0.
+ elim H3; intros; clear H3.
+ substs.
+ elim H2; intros; clear H2.
+ inversion H3.
+ substs.
+ left. 
+ apply fork_tau_behave_ee in H4.
+ destruct H4.
+ destruct H2; destruct H2.
+ exists x1. splits. apply lab_r with (e1:=x)(e2:=e''0)(s:=s0).
+ splits; [ assumption | assumption |  intuition ].
+ substs.
+ intuition.
+ substs.
+ left.
+ exists x2; splits; [ apply star_trans with (y:=x0); [ assumption | assumption ] | reflexivity ].
+ destruct H2; destruct H2.
+ destruct H2.
+ exists x1. splits. apply lab_r with (e1:=x)(e2:=e''0)(s:=s0).
+ splits; [ assumption | assumption |  intuition ].
+ substs.
+ intuition.
+ substs.
+ right; left.
+ exists x2; splits; [ assumption | apply star_trans with (y:=x0); [ assumption | assumption ] | reflexivity ].
+ destruct H2; destruct H2.
+ exists x1. splits. apply lab_r with (e1:=x)(e2:=e''0)(s:=s0).
+ splits; [ assumption | assumption |  intuition ].
+ substs.
+ intuition.
+ substs.
+ right; right; left.
+ exists x2; splits; [ assumption | assumption | apply star_trans with (y:=x0); [ assumption | assumption ] | reflexivity ].
+ destruct H2; destruct H2.
+ exists x1. splits. apply lab_r with (e1:=x)(e2:=e''0)(s:=s0).
+ splits; [ assumption | assumption |  intuition ].
+ substs.
+ intuition.
+ substs.
+ right; right; right.
+ exists x2; splits; [ assumption | apply star_trans with (y:=x0); [ assumption | assumption ] | reflexivity ].
+ substs.
+
+
+ right.
+ 
+ apply fork_tau_behave_ee in H4.
+ destruct H4.
+ destruct H2; destruct H2.
+ exists x2. splits. apply lab_r with (e1:=x0)(e2:=e''0)(s:=s0).
+ splits; [ assumption | assumption |  intuition ].
+ substs.
+ intuition.
+ substs.
+ left.
+ exists x1; splits; [ apply star_trans with (y:=x); [ assumption | assumption ] | reflexivity ].
+ destruct H2; destruct H2.
+ destruct H2.
+ exists x2. splits. apply lab_r with (e1:=x0)(e2:=e''0)(s:=s0).
+ splits; [ assumption | assumption |  intuition ].
+ substs.
+ intuition.
+ substs.
+ right; left.
+ exists x1; splits; [ assumption | apply star_trans with (y:=x); [ assumption | assumption ] | reflexivity ].
+ destruct H2; destruct H2.
+ exists x2. splits. apply lab_r with (e1:=x0)(e2:=e''0)(s:=s0).
+ splits; [ assumption | assumption |  intuition ].
+ substs.
+ intuition.
+ substs.
+ right; right; left.
+ exists x1; splits; [ assumption | assumption | apply star_trans with (y:=x); [ assumption | assumption ] | reflexivity ].
+ destruct H2; destruct H2.
+ exists x2. splits. apply lab_r with (e1:=x0)(e2:=e''0)(s:=s0).
+ splits; [ assumption | assumption |  intuition ].
+ substs.
+ intuition.
+ substs.
+ right; right; right.
+ exists x1; splits; [ assumption | apply star_trans with (y:=x); [ assumption | assumption ] | reflexivity ].
+ substs.
+ 
+
+ apply red_not_value in H9; simpl in H9; intuition.
+ substs.
+ apply red_not_value in H10; simpl in H10; intuition.
+ substs.
+ elim H2; intros; clear H2.
+ apply red_not_value in H1.
+ destruct H0.
+ destruct H0; destruct H0; intuition; substs; simpl in H1; intuition. 
+ destruct H0.
+ destruct H0; destruct H0; intuition; substs; simpl in H1; intuition.
+ destruct H0; destruct H0; intuition; substs; simpl in H1; intuition.
+Qed.
+
+Lemma taured_val_id : forall (e e' : expr), tauRed e e' -> is_value_of_expr e -> e = e'.
+Proof.
+ intros.
+ inversion H.
+ reflexivity.
+ inversion H1.
+ apply red_not_value in H5; contradiction.
+Qed.
+
+Lemma labred_not_val : forall (e e' : expr)(l : label), labRed l e e' -> ~(is_value_of_expr e).
+Proof.
  intros.
  inversion H.
  intuition.
- inversion H4.
- rewrite <- H7 in H0.
+ apply taured_val_id in H5; intuition; substs.
+ apply red_not_value in H0.
+ contradiction.
+Qed. 
+
+
+Check star_ind.
+
+Lemma bind_tau_behave_front : forall ( e e' x : expr), tauRed e x -> tauRed (e >>= e') (x >>= e').
+Proof.
+ intros.
+ apply star_ind with (R:=tauStep)(X:=expr)(P:= (fun y z => tauRed (y >>= e') (z >>= e'))).
+ intros.
+ apply star_refl.
+ intros.
+ apply S_star with (y:=(y>>=e')).
  inversion H0.
- exists ((E_apply
-        (E_apply (E_constant CONST_fork)
-           (E_live_expr ( (LM_comp rl0))))
-        (E_live_expr (LM_expr (E_constant CONST_unit)))) >>= swapf).
- split.
- rewrite <- H12 in H6.
- apply lab_r.
+ apply tStep with (s:= s).
+ apply JO_red_evalbind.
+ assumption.
+ assumption.
+ assumption.
+Qed.
+
+Lemma bind_lab_behave_front : forall ( e e' x : expr) (l : label), labRed l e x -> labRed l (e >>= e') (x >>= e').
+Proof.
+ intros.
+ inversion H.
+ intuition.
+ substs.
+ apply lab_r with (e1:=(e1 >>= e'))(e2:=(e2 >>= e'))(s:=s).
+ splits; [apply bind_tau_behave_front; assumption | apply JO_red_evalbind; assumption | apply bind_tau_behave_front; assumption ].
+Qed.
+
+Lemma fork_tau_behave_edge1 : forall  (e e' x : expr), tauRed e x -> ~ (is_value_of_expr e') -> tauRed (E_apply (E_apply (E_constant CONST_fork) (E_live_expr (LM_expr e))) (E_live_expr (LM_expr e'))) (E_apply (E_apply (E_constant CONST_fork) (E_live_expr (LM_expr x))) (E_live_expr (LM_expr e'))).
+Proof. 
+ intros.
+ apply star_ind with (R:=tauStep)(X:=expr)(P:= (fun y z => tauRed (E_apply (E_apply (E_constant CONST_fork) (E_live_expr (LM_expr y))) (E_live_expr (LM_expr e'))) (E_apply (E_apply (E_constant CONST_fork) (E_live_expr (LM_expr z))) (E_live_expr (LM_expr e'))))).
+ intros; apply star_refl.
+ intros.
+ apply S_star with (y:=(E_apply (E_apply (E_constant CONST_fork) (E_live_expr (LM_expr y))) (E_live_expr (LM_expr e')))).
+ apply tStep with (s:=S_First).
+ inversion H1.
+ apply  JO_red_forkmove1 with (s:=s).
+ assumption.
+ assumption.
+ assumption.
+ assumption.
+Qed.
+
+Lemma fork_tau_behave_edge2 : forall  (e e' x : expr), tauRed e' x -> ~ (is_value_of_expr e) -> tauRed (E_apply (E_apply (E_constant CONST_fork) (E_live_expr (LM_expr e))) (E_live_expr (LM_expr e'))) (E_apply (E_apply (E_constant CONST_fork) (E_live_expr (LM_expr e))) (E_live_expr (LM_expr x))).
+Proof. 
+ intros.
+ apply star_ind with (R:=tauStep)(X:=expr)(P:= (fun y z => tauRed (E_apply (E_apply (E_constant CONST_fork) (E_live_expr (LM_expr e))) (E_live_expr (LM_expr y))) (E_apply (E_apply (E_constant CONST_fork) (E_live_expr (LM_expr e))) (E_live_expr (LM_expr z))))).
+ intros; apply star_refl.
+ intros.
+ apply S_star with (y:=(E_apply (E_apply (E_constant CONST_fork) (E_live_expr (LM_expr e))) (E_live_expr (LM_expr y)))).
+ apply tStep with (s:=S_Second).
+ inversion H1.
+ apply  JO_red_forkmove2 with (s:=s).
+ assumption.
+ assumption.
+ assumption.
+ assumption.
+Qed.
+
+Lemma fork_lab_behave_edge1 : forall  (e e' x : expr) (l:label), labRed l e x -> ~ (is_value_of_expr e') -> labRed l (E_apply (E_apply (E_constant CONST_fork) (E_live_expr (LM_expr e))) (E_live_expr (LM_expr e'))) (E_apply (E_apply (E_constant CONST_fork) (E_live_expr (LM_expr x))) (E_live_expr (LM_expr e'))).
+Proof.
+ intros.
+ inversion H.
+ intuition.
+ substs.
+ apply lab_r with (e1:= (E_apply (E_apply (E_constant CONST_fork) (E_live_expr (LM_expr e1)))
+     (E_live_expr (LM_expr e'))))(e2:= (E_apply (E_apply (E_constant CONST_fork) (E_live_expr (LM_expr e2)))
+     (E_live_expr (LM_expr e'))))(s:=S_First).
+ splits.
+ apply fork_tau_behave_edge1;[ assumption | assumption ].
+ apply JO_red_forkmove1 with (s:=s); [ assumption |  assumption ].
+ apply fork_tau_behave_edge1; [ assumption |  assumption ].
+Qed.
+
+Lemma fork_tau_behave_edge12 : forall  (e e' x y : expr), tauRed e' x -> tauRed e y -> ~ is_value_of_expr e' -> ~ (is_value_of_expr e) -> ~ is_value_of_expr y -> ~ (is_value_of_expr x) -> tauRed (E_apply (E_apply (E_constant CONST_fork) (E_live_expr (LM_expr e))) (E_live_expr (LM_expr e'))) (E_apply (E_apply (E_constant CONST_fork) (E_live_expr (LM_expr y))) (E_live_expr (LM_expr x))).
+Proof. 
+ intros.
+ assert (He:=H0).
+ apply fork_tau_behave_edge1 with (e':=e') in He.
+ assert (He':=H).
+ apply fork_tau_behave_edge2 with (e:=y) in He'.
+ apply star_trans with (y:=(E_apply (E_apply (E_constant CONST_fork) (E_live_expr (LM_expr y)))
+          (E_live_expr (LM_expr e')))).
+ assumption.
+ assumption.
+ assumption.
+ assumption.
+Qed.
+
+
+
+
+Lemma fork_lab_behave_edge2 : forall  (e e' x : expr) (l:label), labRed l e' x -> ~ (is_value_of_expr e) -> labRed l (E_apply (E_apply (E_constant CONST_fork) (E_live_expr (LM_expr e))) (E_live_expr (LM_expr e'))) (E_apply (E_apply (E_constant CONST_fork) (E_live_expr (LM_expr e))) (E_live_expr (LM_expr x))).
+Proof.
+ intros.
+ inversion H.
+ intuition.
+ substs.
+ apply lab_r with (e1:= (E_apply (E_apply (E_constant CONST_fork) (E_live_expr (LM_expr e)))
+     (E_live_expr (LM_expr e1))))(e2:= (E_apply (E_apply (E_constant CONST_fork) (E_live_expr (LM_expr e)))
+     (E_live_expr (LM_expr e2))))(s:=S_Second).
+ splits.
+ apply fork_tau_behave_edge2;[ assumption | assumption ].
+ apply JO_red_forkmove2 with (s:=s); [ assumption |  assumption ].
+ apply fork_tau_behave_edge2; [ assumption |  assumption ].
+Qed.
+
+Lemma fork_tau_serialise1 : forall (p q p' q': expr), tauRed
+       (E_apply (E_apply (E_constant CONST_fork) (E_live_expr (LM_expr p)))
+          (E_live_expr (LM_expr q)))
+       (E_apply (E_apply (E_constant CONST_fork) (E_live_expr (LM_expr p')))
+          (E_live_expr (LM_expr q'))) -> tauRed
+       (E_apply (E_apply (E_constant CONST_fork) (E_live_expr (LM_expr p)))
+          (E_live_expr (LM_expr q)))
+       (E_apply (E_apply (E_constant CONST_fork) (E_live_expr (LM_expr p')))
+          (E_live_expr (LM_expr q))).
+Proof.
+ intros.
+ assert (H0 := H).
+ apply fork_tau_behave_ee in H0.
+ intuition.
+ destruct H1.
+ destruct H0.
+ intuition.
+ simplify_eq H3.
+ intros; substs.
+ clear H3.
+ inversion H.
+ substs.
+ apply star_refl.
+ substs.
+ inversion H2.
+ substs.
+ inversion H4.
+ substs.
+ apply fork_tau_behave_edge1.
+ assumption.
+ assumption.
+ substs.
+ apply fork_tau_behave_edge1.
+ assumption.
+ apply red_not_value in H11.
+ assumption.
+ substs.
+ inversion H3.
+ substs.
+ inversion H5.
+ apply red_not_value in H7; simpl in H7; intuition.
+ substs.
+ inversion H3.
+ substs.
+ inversion H5.
+ apply red_not_value in H7; simpl in H7; intuition.
+ substs.
+ inversion H3.
+ substs.
+ inversion H5.
+ apply red_not_value in H8; simpl in H8; intuition.
+ substs.
+ apply red_not_value in H10; simpl in H10; intuition.
+ substs.
+ apply red_not_value in H11; simpl in H11; intuition.
+ substs.
+ destruct H0.
+ destruct H0.
+ intuition.
+ discriminate H4.
+ destruct H1.
+ destruct H0.
+ intuition.
+ discriminate H5.
+ destruct H1; destruct H0; intuition.
+ discriminate H4.
+Qed.
  
-Admitted. 
-*)
+
+Lemma fork_tau_swap_ee_non_val : forall (p q p' q': expr), (~ (is_value_of_expr p)) -> (~(is_value_of_expr q)) ->  (~ (is_value_of_expr p')) -> (~(is_value_of_expr q')) ->  tauRed
+       (E_apply (E_apply (E_constant CONST_fork) (E_live_expr (LM_expr p)))
+          (E_live_expr (LM_expr q)))
+       (E_apply (E_apply (E_constant CONST_fork) (E_live_expr (LM_expr p')))
+          (E_live_expr (LM_expr q'))) -> tauRed
+       (E_apply (E_apply (E_constant CONST_fork) (E_live_expr (LM_expr q)))
+          (E_live_expr (LM_expr p)))
+       (E_apply (E_apply (E_constant CONST_fork) (E_live_expr (LM_expr q')))
+          (E_live_expr (LM_expr p'))).
+Proof.
+ intros.
+ apply fork_tau_behave_ee in H3.
+ intuition.
+ destruct H4; destruct H3; intuition.
+ simplify_eq H6; intros; substs.
+ apply fork_tau_behave_edge12.
+ assumption. assumption. assumption. assumption. assumption. assumption.
+ destruct H3; destruct H3; intuition.
+ simplify_eq H7; intros; substs.
+ destruct H4; destruct H3; intuition.
+ simplify_eq H8; intros; substs; assumption.
+ destruct H4; destruct H3; intuition.
+ simplify_eq H7; intros; substs; assumption.
+Qed.
+
+
+Lemma star_rev_ind : forall (X :Type) (R: relation X) (P : X -> X -> Prop),
+      (forall x : X, P x x) ->
+       (forall y x z : X, star R x y -> R y z -> P x y -> P x z) ->
+       forall x x0 : X, star R x x0 -> P x x0.
+Proof.
+ intros.
+ assert (star ( trans R ) x0 x).
+ assert ((trans ( star R) ) x0 x).
+ unfold trans.
+ assumption.
+ assert (eeq (trans (star R)) (star (trans R))).
+ apply inv_star.
+ intuition.
+ unfold eeq in H3.
+ intuition.
+ assert (H3:=H2).
+ induction H2.
+ apply H.
+ substs.
+ apply H0 with (y:=y).
+ assert ((trans ( star R) ) y z).
+ assert (eeq (trans (star R)) (star (trans R))).
+ apply inv_star.
+ intuition.
+ unfold eeq in H5.
+ intuition.
+ unfold trans in H5.
+ assumption.
+ unfold trans in H2.
+ assumption.
+ apply IHstar.
+ assert ((trans ( star R) ) y z).
+ assert (eeq (trans (star R)) (star (trans R))).
+ apply inv_star.
+ intuition.
+ unfold eeq in H5.
+ intuition.
+ unfold trans in H5.
+ assumption.
+ assumption.
+Qed.
+
+
+Lemma fork_comm_step_int : forall (p q p' q' : livemodes) (s: select)(rl : redlabel), (E_apply (E_apply (E_constant CONST_fork) (E_live_expr (p))) (E_live_expr (q))) [ s ] --> [ rl ] (E_apply (E_apply (E_constant CONST_fork) (E_live_expr (p'))) (E_live_expr (q'))) ->
+(exists (s' : select ), (E_apply (E_apply (E_constant CONST_fork) (E_live_expr (q))) (E_live_expr (p))) [ s' ] --> [ rl ] (E_apply (E_apply (E_constant CONST_fork) (E_live_expr (q'))) (E_live_expr (p')))).
+Proof.
+ intros.
+ inversion H.
+ substs.
+ exists (S_Second).
+ apply JO_red_forkmove2 with (s:=s0).
+ assumption. assumption.
+ substs.
+ exists (S_First).
+ apply JO_red_forkmove1 with (s:=s0).
+ assumption. assumption.
+ substs.
+ exists (S_Second).
+ apply JO_red_forkdocomp21.
+ substs.
+ exists (S_First).
+ apply JO_red_forkdocomp12.
+ substs.
+ apply red_not_value in H4; simpl in H4; intuition.
+ substs.
+ apply red_not_value in H7; simpl in H7; intuition.
+Qed.
+
+Lemma fork_comm_taustep : forall (p q p' q' : livemodes), tauStep (E_apply (E_apply (E_constant CONST_fork) (E_live_expr (p))) (E_live_expr (q))) (E_apply (E_apply (E_constant CONST_fork) (E_live_expr (p'))) (E_live_expr (q'))) -> 
+                          tauStep (E_apply (E_apply (E_constant CONST_fork) (E_live_expr (q))) (E_live_expr (p))) (E_apply (E_apply (E_constant CONST_fork) (E_live_expr (q'))) (E_live_expr (p'))).
+Proof. 
+intros.
+ inversion H.
+ substs.
+ apply fork_comm_step_int in H0.
+ destruct H0.
+ apply tStep with (s:=x).
+ assumption.
+Qed.
+
+Lemma fork_comm_taured_h : forall (x y : expr), tauRed x y -> ((fun x y => (exists (p q p' q' : livemodes), x = (E_apply (E_apply (E_constant CONST_fork) (E_live_expr p))
+         (E_live_expr q)) /\ y = (E_apply (E_apply (E_constant CONST_fork) (E_live_expr p'))
+         (E_live_expr q'))) -> (exists (p q p' q' : livemodes), x = (E_apply (E_apply (E_constant CONST_fork) (E_live_expr p))
+         (E_live_expr q)) /\ y = (E_apply (E_apply (E_constant CONST_fork) (E_live_expr p'))
+         (E_live_expr q')) /\ tauRed
+  (E_apply (E_apply (E_constant CONST_fork) (E_live_expr q)) (E_live_expr p))
+  (E_apply (E_apply (E_constant CONST_fork) (E_live_expr q'))     (E_live_expr p')))) x y).
+Proof.
+ apply star_ind.
+ intros.
+ destruct H; destruct H; destruct H; destruct H.
+ intuition.
+ substs.
+ simplify_eq H1.
+ intros; substs.
+ exists x2 x3 x2 x3.
+ splits.
+ reflexivity.
+ reflexivity.
+ apply star_refl.
+ intros.
+ intuition. 
+ destruct H2. destruct H2; destruct H2; destruct H2.
+ intuition; substs.
+ exists x0 x1 x2 x3.
+ splits.
+ reflexivity.
+ reflexivity.
+ inversion H.
+ substs.
+ inversion H2.
+ intros.
+ substs.
+ assert (exists p q p' q',
+     E_apply (E_apply (E_constant CONST_fork) (E_live_expr (LM_expr e'')))
+       (E_live_expr (LM_expr e')) =
+     E_apply (E_apply (E_constant CONST_fork) (E_live_expr p))
+       (E_live_expr q) /\
+     E_apply (E_apply (E_constant CONST_fork) (E_live_expr x2))
+       (E_live_expr x3) =
+     E_apply (E_apply (E_constant CONST_fork) (E_live_expr p'))
+       (E_live_expr q') /\
+     tauRed
+       (E_apply (E_apply (E_constant CONST_fork) (E_live_expr q))
+          (E_live_expr p))
+       (E_apply (E_apply (E_constant CONST_fork) (E_live_expr q'))
+          (E_live_expr p'))).
+ apply H1.
+ exists (LM_expr e'') (LM_expr e') x2 x3.
+ splits; [reflexivity | reflexivity].
+ destruct H3. destruct H3; destruct H3; destruct H3.
+ intuition.
+ simplify_eq H4.
+ simplify_eq H3.
+ intros.
+ substs.
+ clear H3.
+ clear H4.
+ apply S_star with (y:=((E_apply (E_apply (E_constant CONST_fork) (E_live_expr (LM_expr e')))
+          (E_live_expr (LM_expr e''))))).
+ apply tStep with (s:=S_Second).
+ apply JO_red_forkmove2 with (s:=s0).
+ intuition.
+ assumption.
+ assumption.
+ substs.
+ assert (exists p q p' q',
+     E_apply (E_apply (E_constant CONST_fork) (E_live_expr (LM_expr e)))
+       (E_live_expr (LM_expr e'')) =
+     E_apply (E_apply (E_constant CONST_fork) (E_live_expr p))
+       (E_live_expr q) /\
+     E_apply (E_apply (E_constant CONST_fork) (E_live_expr x2))
+       (E_live_expr x3) =
+     E_apply (E_apply (E_constant CONST_fork) (E_live_expr p'))
+       (E_live_expr q') /\
+     tauRed
+       (E_apply (E_apply (E_constant CONST_fork) (E_live_expr q))
+          (E_live_expr p))
+       (E_apply (E_apply (E_constant CONST_fork) (E_live_expr q'))
+          (E_live_expr p'))).
+ apply H1.
+ exists (LM_expr e) (LM_expr e'') x2 x3.
+ splits; [reflexivity | reflexivity ].
+ destruct H3; destruct H3; destruct H3; destruct H3.
+ intuition.
+ substs.
+ simplify_eq H4; simplify_eq H3; intros; substs; clear H4; clear H3.
+ apply S_star with (y:=((E_apply (E_apply (E_constant CONST_fork) (E_live_expr (LM_expr e'')))
+     (E_live_expr (LM_expr e))))).
+ apply tStep with (s:=S_First).
+ apply JO_red_forkmove1 with (s:=s0).
+ assumption.
+ assumption.
+ assumption.
+ substs.
+ inversion H0.
+ substs.
+ inversion H3.
+ substs.
+ apply red_not_value in H5; simpl in H5; intuition.
+ substs.
+ inversion H0.
+ substs.
+ inversion H3.
+ substs.
+ apply red_not_value in H5; simpl in H5; intuition.
+ substs.
+ inversion H0.
+ substs.
+ inversion H3.
+ substs.
+ apply red_not_value in H6; simpl in H6; intuition.
+ substs.
+ apply red_not_value in H8; simpl in H8; intuition.
+ substs.
+ apply red_not_value in H9; simpl in H9; intuition.
+Qed.
+
+Lemma fork_comm_taured : forall (p q p' q' : livemodes), tauRed (E_apply (E_apply (E_constant CONST_fork) (E_live_expr (p))) (E_live_expr (q))) (E_apply (E_apply (E_constant CONST_fork) (E_live_expr (p'))) (E_live_expr (q'))) -> 
+                          tauRed (E_apply (E_apply (E_constant CONST_fork) (E_live_expr (q))) (E_live_expr (p))) (E_apply (E_apply (E_constant CONST_fork) (E_live_expr (q'))) (E_live_expr (p'))).
+Proof.
+ intros.
+ apply fork_comm_taured_h in H.
+ destruct H;destruct H;destruct H;destruct H.
+ intuition.
+ simplify_eq H0; simplify_eq H; intros; substs; clear H0; clear H.
+ assumption.
+ exists p q p' q'; splits ; [reflexivity | reflexivity ].
+Qed.
+
+Lemma fork_comm_labred : forall (p q p' q' : livemodes)(l :label), labRed l (E_apply (E_apply (E_constant CONST_fork) (E_live_expr (p))) (E_live_expr (q))) (E_apply (E_apply (E_constant CONST_fork) (E_live_expr (p'))) (E_live_expr (q'))) -> 
+                          labRed l (E_apply (E_apply (E_constant CONST_fork) (E_live_expr (q))) (E_live_expr (p))) (E_apply (E_apply (E_constant CONST_fork) (E_live_expr (q'))) (E_live_expr (p'))).
+Proof.
+ intros.
+ inversion H.
+ substs.
+ intuition.
+ induction p.
+ induction q.
+ apply fork_tau_behave_cc in H1.
+ substs.
+ inversion H0.
+ intros. 
+ substs.
+ apply lab_r with (e1:=(E_apply (E_apply (E_constant CONST_fork) (E_live_expr (LM_comp lab0)))
+     (E_live_expr (LM_comp l))))(e2:=(E_apply (E_apply (E_constant CONST_fork) (E_live_expr (LM_comp lab0)))
+     (E_live_expr (LM_expr (E_constant CONST_unit)))))(s:=S_Second).
+ splits.
+ apply star_refl.
+ apply JO_red_forkdocomp21.
+ apply fork_comm_taured.
+ assumption.
+ substs.
+ apply lab_r with (e1:=(E_apply (E_apply (E_constant CONST_fork) (E_live_expr (LM_comp l)))
+     (E_live_expr (LM_comp lab))))(e2:=(E_apply (E_apply (E_constant CONST_fork) (E_live_expr (LM_expr (E_constant CONST_unit))))
+     (E_live_expr (LM_comp lab))))(s:=S_First).
+ splits.
+ apply star_refl.
+ apply JO_red_forkdocomp12.
+ apply fork_comm_taured.
+ assumption.
+ substs.
+ apply red_not_value in H7; simpl in H7; intuition.
+ substs.
+ apply red_not_value in H8; simpl in H8; intuition.
+ substs.
+  apply fork_tau_behave_ce in H1.
+ substs.
+ inversion H0.
+ substs.
+ apply taured_val_id in H3. discriminate H3.
+ simpl; auto.
+ substs.
+ apply taured_val_id in H3. discriminate H3.
+ simpl; auto.
+ substs.
+ apply red_not_value in H7; simpl in H7; intuition.
+ substs.
+ apply red_not_value in H8; simpl in H8; intuition.
+ substs.
+ induction q.
+ apply fork_tau_behave_ec in H1.
+ substs.
+  inversion H0.
+ substs.
+ apply taured_val_id in H3. discriminate H3.
+ simpl; auto.
+ substs.
+ apply taured_val_id in H3. discriminate H3.
+ simpl; auto.
+ substs.
+ apply red_not_value in H7; simpl in H7; intuition.
+ substs.
+ apply red_not_value in H8; simpl in H8; intuition.
+ substs.
+ assert (K:=H1).
+ apply fork_tau_behave_ee in H1.
+ intuition.
+ destruct H2. destruct H1.
+ intuition.
+ substs.
+ inversion H0.
+ substs.
+  apply lab_r with (e1:=(E_apply (E_apply (E_constant CONST_fork) (E_live_expr (LM_expr x0)))
+       (E_live_expr (LM_expr x))))(e2:=(E_apply (E_apply (E_constant CONST_fork) (E_live_expr (LM_expr x0)))
+       (E_live_expr (LM_expr e''))))(s:=S_Second).
+ substs.
+ splits.
+ apply fork_comm_taured.
+ assumption.
+ apply JO_red_forkmove2 with (s:=s0).
+ assumption.
+ assumption.
+ apply fork_comm_taured.
+ assumption.
+ substs.
+ apply lab_r with (e1:=(E_apply (E_apply (E_constant CONST_fork) (E_live_expr (LM_expr x0)))
+       (E_live_expr (LM_expr x))))(e2:=(E_apply (E_apply (E_constant CONST_fork) (E_live_expr (LM_expr e'')))
+       (E_live_expr (LM_expr x))))(s:=S_First).
+ substs.
+ splits.
+ apply fork_comm_taured.
+ assumption.
+ apply JO_red_forkmove1 with (s:=s0).
+ assumption.
+ assumption.
+ apply fork_comm_taured.
+ assumption.
+ apply red_not_value in H9; simpl in H9; intuition.
+ apply red_not_value in H10; simpl in H10; intuition.
+ destruct H1; destruct H1.
+ intuition.
+ substs.
+ apply red_not_value in H0; simpl in H0; intuition.
+ destruct H2; destruct H1.
+ intuition.
+ substs.
+ apply red_not_value in H0; simpl in H0; intuition.
+ destruct H2; destruct H1.
+ intuition.
+ substs.
+ apply red_not_value in H0; simpl in H0; intuition.
+Qed.
+
+Lemma fork_lab_behave : forall (p q : livemodes)(e : expr)(l : label),  labRed l (E_apply (E_apply (E_constant CONST_fork) (E_live_expr (p))) (E_live_expr (q)))  e ->
+ ((exists (p' q' : livemodes), e=(E_apply (E_apply (E_constant CONST_fork) (E_live_expr (p'))) (E_live_expr (q'))) ) \/ 
+
+(exists (lm : livemodes), e=(E_live_expr lm)) /\ 
+(exists (p' q' : livemodes), ((exists (s : select), (E_apply (E_apply (E_constant CONST_fork) (E_live_expr (p')) ) (E_live_expr (q'))) [ s ] --> [ RL_labelled l ] e)  /\ tauRed (E_apply (E_apply (E_constant CONST_fork) (E_live_expr (p))) (E_live_expr (q))) (E_apply (E_apply (E_constant CONST_fork) (E_live_expr (p'))) (E_live_expr (q')))) 
+    \/ (labRed l (E_apply (E_apply (E_constant CONST_fork) (E_live_expr (p)) ) (E_live_expr (q)))  (E_apply (E_apply (E_constant CONST_fork) (E_live_expr (p')) ) (E_live_expr (q'))) /\ tauRed (E_apply (E_apply (E_constant CONST_fork) (E_live_expr (p')) ) (E_live_expr (q'))) e)) ).
+intros.
+ inversion H.
+ substs.
+ intuition.
+ induction p; induction q.
+ apply fork_tau_behave_cc in H1.
+ substs.
+ inversion H0.
+ substs.
+ apply fork_tau_behave_ec in H3.
+ substs.
+ left.
+ exists (LM_expr (E_constant CONST_unit)) (LM_comp lab0); reflexivity.
+ substs.
+ apply fork_tau_behave_ce in H3.
+ substs.
+ left.
+ exists   (LM_comp lab) (LM_expr (E_constant CONST_unit)); reflexivity.
+ substs.
+ apply red_not_value in H7; simpl in H7; intuition.
+ substs.
+ apply red_not_value in H8; simpl in H8; intuition.
+ substs.
+ apply fork_tau_behave_ce in H1.
+ substs.
+ inversion H0.
+ substs.
+ apply taured_val_id in H3.
+ substs. 
+ right.
+ splits.
+ exists (LM_expr
+     (E_taggingleft
+        (E_taggingright
+           (E_pair (E_constant CONST_unit) (E_live_expr (LM_expr expr5)))))); reflexivity.
+ simpl; auto.
+ exists (LM_comp l) (LM_expr expr5).
+ left.
+ splits.
+ exists s.
+ assumption.
+ apply star_refl.
+ simpl.
+ auto.
+ substs.
+ apply taured_val_id in H3.
+ substs. 
+ right.
+ splits.
+ exists (LM_expr
+     (E_taggingleft
+        (E_taggingleft
+           (E_pair (E_constant CONST_unit) (E_constant CONST_unit))))); reflexivity.
+ simpl; auto.
+ exists (LM_comp l) (LM_expr (E_constant CONST_unit)).
+ left.
+ splits.
+ exists s.
+ assumption.
+ apply star_refl.
+ simpl.
+ auto.
+ substs.
+ apply red_not_value in H7; simpl in H7; intuition.
+ apply red_not_value in H8; simpl in H8; intuition.
+ apply fork_tau_behave_ec in H1.
+ substs.
+ inversion H0.
+ substs.
+ apply taured_val_id in H3.
+ substs. 
+ right.
+ splits.
+ exists (LM_expr
+     (E_taggingright
+        (E_pair (E_live_expr (LM_expr expr5)) (E_constant CONST_unit)))); reflexivity.
+ simpl; auto.
+ exists (LM_expr expr5) (LM_comp l).
+ left.
+ splits.
+ exists s.
+ assumption.
+ apply star_refl.
+ simpl.
+ auto.
+ substs.
+ apply taured_val_id in H3.
+ substs. 
+ right.
+ splits.
+ exists (LM_expr
+     (E_taggingleft
+        (E_taggingleft
+           (E_pair (E_constant CONST_unit) (E_constant CONST_unit))))); reflexivity.
+ simpl; auto.
+  exists (LM_expr (E_constant CONST_unit)) (LM_comp l).
+ left.
+ splits.
+ exists s.
+ assumption.
+ apply star_refl.
+ simpl.
+ auto.
+ 
+ substs.
+  apply red_not_value in H7; simpl in H7; intuition.
+ apply red_not_value in H8; simpl in H8; intuition.
+ assert (K:=H1).
+ apply fork_tau_behave_ee in H1.
+ intuition.
+ destruct H2; destruct H1.
+ intuition.
+ substs.
+ inversion H0.
+ substs.
+ assert (L:=H3).
+ apply fork_tau_behave_ee in H3.
+ intuition.
+ left.
+ destruct H4. destruct H3.
+ intuition; substs; exists (LM_expr x1) (LM_expr x2); reflexivity.
+ right.
+ destruct H3. destruct H3.
+ intuition; substs.
+ exists (LM_expr (E_taggingright (E_pair (E_live_expr (LM_expr x1)) x2))); reflexivity.
+ exists ( (LM_expr e'')) (LM_expr x0).
+ right.
+ splits.
+ apply lab_r with (e1:=(E_apply (E_apply (E_constant CONST_fork) (E_live_expr (LM_expr x)))
+         (E_live_expr (LM_expr x0))))(e2:=(E_apply (E_apply (E_constant CONST_fork) (E_live_expr (LM_expr e'')))
+       (E_live_expr (LM_expr x0))))(s:=S_First).
+ splits; [ assumption | assumption | apply star_refl ].
+ assumption.
+  destruct H4. destruct H3.
+ right.
+ intuition; substs.
+  exists (LM_expr (E_taggingleft (E_taggingleft (E_pair x1 x2)))); reflexivity.
+ exists ( (LM_expr e'')) (LM_expr x0).
+ right.
+ splits.
+ apply lab_r with (e1:=(E_apply (E_apply (E_constant CONST_fork) (E_live_expr (LM_expr x)))
+         (E_live_expr (LM_expr x0))))(e2:=(E_apply (E_apply (E_constant CONST_fork) (E_live_expr (LM_expr e'')))
+       (E_live_expr (LM_expr x0))))(s:=S_First).
+ splits; [ assumption | assumption | apply star_refl ].
+ assumption.
+   destruct H4. destruct H3.
+ right.
+ intuition; substs.
+ exists (LM_expr
+          (E_taggingleft
+             (E_taggingright (E_pair x1 (E_live_expr (LM_expr x2)))))); reflexivity.
+ exists ( (LM_expr e'')) (LM_expr x0).
+ right.
+ splits.
+ apply lab_r with (e1:=(E_apply (E_apply (E_constant CONST_fork) (E_live_expr (LM_expr x)))
+         (E_live_expr (LM_expr x0))))(e2:=(E_apply (E_apply (E_constant CONST_fork) (E_live_expr (LM_expr e'')))
+       (E_live_expr (LM_expr x0))))(s:=S_First).
+ splits; [ assumption | assumption | apply star_refl ].
+ assumption.
+ substs.
+ assert (L:=H3).
+ apply fork_tau_behave_ee in H3.
+ intuition.
+ destruct H4; destruct H3.
+ intuition.
+ substs.
+ left.
+ intuition; substs; exists (LM_expr x1) (LM_expr x2); reflexivity.
+ right.
+ destruct H3. destruct H3.
+ intuition; substs.
+ exists (LM_expr (E_taggingright (E_pair (E_live_expr (LM_expr x1)) x2))); reflexivity.
+ exists ( (LM_expr x)) (LM_expr e'').
+ right.
+ splits.
+ apply lab_r with (e1:=(E_apply (E_apply (E_constant CONST_fork) (E_live_expr (LM_expr x)))
+         (E_live_expr (LM_expr x0))))(e2:=(E_apply (E_apply (E_constant CONST_fork) (E_live_expr (LM_expr x)))
+       (E_live_expr (LM_expr e''))))(s:=S_Second).
+ splits; [ assumption | assumption | apply star_refl ].
+ assumption.
+  destruct H4. destruct H3.
+ right.
+ intuition; substs.
+ exists (LM_expr (E_taggingleft (E_taggingleft (E_pair x1 x2)))); reflexivity.
+ exists ( (LM_expr x)) (LM_expr e'').
+ right.
+ splits.
+ apply lab_r with (e1:=(E_apply (E_apply (E_constant CONST_fork) (E_live_expr (LM_expr x)))
+         (E_live_expr (LM_expr x0))))(e2:=(E_apply (E_apply (E_constant CONST_fork) (E_live_expr (LM_expr x)))
+       (E_live_expr (LM_expr e''))))(s:=S_Second).
+ splits; [ assumption | assumption | apply star_refl ].
+ assumption.
+   destruct H4. destruct H3.
+ right.
+ intuition; substs.
+ exists (LM_expr
+          (E_taggingleft
+             (E_taggingright (E_pair x1 (E_live_expr (LM_expr x2)))))); reflexivity.
+ exists ( (LM_expr x)) (LM_expr e'').
+ right.
+ splits.
+ apply lab_r with (e1:=(E_apply (E_apply (E_constant CONST_fork) (E_live_expr (LM_expr x)))
+         (E_live_expr (LM_expr x0))))(e2:=(E_apply (E_apply (E_constant CONST_fork) (E_live_expr (LM_expr x)))
+       (E_live_expr (LM_expr e''))))(s:=S_Second).
+ splits; [ assumption | assumption | apply star_refl ].
+ assumption.
+ substs.
+ apply red_not_value in H9; simpl in H9; intuition.
+ apply red_not_value in H10; simpl in H10; intuition.
+ destruct H1; destruct H1; intuition; substs; apply red_not_value in H0; simpl in H0; intuition.
+ destruct H2; destruct H1; intuition; substs; apply red_not_value in H0; simpl in H0; intuition.
+ destruct H2; destruct H1; intuition; substs; apply red_not_value in H0; simpl in H0; intuition.
+Qed.
+
+ 
+
+ 
+
+Lemma fork_comm_step_fin : forall (p q lm : livemodes) (s: select)(rl : redlabel), (E_apply (E_apply (E_constant CONST_fork) (E_live_expr (p))) (E_live_expr (q))) [ s ] --> [ rl ] (E_live_expr lm )->
+(exists (s' : select ) (lm' : livemodes), (E_apply (E_apply (E_constant CONST_fork) (E_live_expr (q))) (E_live_expr (p))) [ s' ] --> [ rl ] (E_live_expr lm') /\ totalTauRed ((E_live_expr lm') >>= swapf) (E_live_expr lm ) ).
+Proof.
+ intros.
+ inversion H.
+ substs.
+ exists s.
+ exists (
+      (LM_expr
+         ((E_taggingright (E_pair  (E_live_expr (LM_expr e)) v))))).
+ splits.
+ apply JO_red_forkdeath2.
+ assumption.
+ apply S_star with (y:= ( E_apply (swapf) (E_taggingright (( E_pair (E_live_expr (LM_expr e))  v )) ) )).
+ apply ttStep.
+ splits.
+ apply tStep with (s:=S_First).
+ apply JO_red_dobind.
+ simpl; auto.
+ intros.
+ inversion H0.
+ substs.
+ apply red_not_value in H7; simpl in H7; intuition.
+ substs.
+ apply red_not_value in H7; simpl in H7; intuition.
+ substs.
+ intros.
+ inversion H0.
+ substs.
+  apply red_not_value in H1; simpl in H1; intuition.
+ inversion H0.
+ substs.
+ inversion H2.
+ substs.
+  apply red_not_value in H9; simpl in H9; intuition.
+ substs.
+ apply red_not_value in H2; simpl in H2; intuition.
+ apply red_not_value in H9; simpl in H9; intuition. 
+ reflexivity.
+ apply swapf_right.
+ simpl; auto.
+ assumption.
+ substs.
+
+  exists s.
+ exists (
+      (LM_expr
+         ((E_taggingleft(E_taggingright (E_pair   v' (E_live_expr (LM_expr e)))))))).
+ splits.
+ apply JO_red_forkdeath1.
+ assumption.
+ apply S_star with (y:= ( E_apply (swapf) (E_taggingleft(E_taggingright (E_pair   v' (E_live_expr (LM_expr e))))) )).
+ apply ttStep.
+ splits.
+ apply tStep with (s:=S_First).
+ apply JO_red_dobind.
+ simpl; auto.
+ intros.
+ inversion H0.
+ substs.
+ apply red_not_value in H7; simpl in H7; intuition.
+ substs.
+ apply red_not_value in H7; simpl in H7; intuition.
+ substs.
+ intros.
+ inversion H0.
+ substs.
+  apply red_not_value in H1; simpl in H1; intuition.
+ inversion H0.
+ substs.
+ inversion H2.
+ substs.
+  apply red_not_value in H9; simpl in H9; intuition.
+ substs.
+ apply red_not_value in H2; simpl in H2; intuition.
+ apply red_not_value in H9; simpl in H9; intuition. 
+ reflexivity.
+ apply swapf_left_right.
+ simpl; auto.
+ simpl; auto.
+ substs.
+
+
+  exists s.
+ exists (
+      (LM_expr
+         ((E_taggingleft(E_taggingleft (E_pair   v' v)))))).
+ splits.
+ apply JO_red_forkdeath12.
+ assumption.
+ assumption.
+ apply S_star with (y:= ( E_apply (swapf) (E_taggingleft(E_taggingleft (E_pair   v' v ))) )).
+ apply ttStep.
+ splits.
+ apply tStep with (s:=S_First).
+ apply JO_red_dobind.
+ simpl; auto.
+ intros.
+ inversion H0.
+ substs.
+ apply red_not_value in H8; simpl in H8; intuition.
+ substs.
+ apply red_not_value in H8; simpl in H8; intuition.
+ substs.
+ intros.
+ inversion H0.
+ substs.
+  apply red_not_value in H1; simpl in H1; intuition.
+ inversion H0.
+ substs.
+ inversion H2.
+ substs.
+  apply red_not_value in H10; simpl in H10; intuition.
+ substs.
+ apply red_not_value in H2; simpl in H2; intuition.
+ apply red_not_value in H10; simpl in H10; intuition. 
+ reflexivity.
+ apply swapf_left_left.
+ simpl; auto.
+ simpl; auto.
+ substs.
+
+
+  exists s.
+ exists (
+      (LM_expr
+         (((E_taggingright (E_pair   (E_live_expr (LM_expr e)) (E_constant CONST_unit))))))).
+ splits.
+ apply JO_red_forkdocomp2.
+ apply S_star with (y:= ( E_apply (swapf) ((E_taggingright (E_pair (E_live_expr (LM_expr e)) (E_constant CONST_unit) ))) )).
+ apply ttStep.
+ splits.
+ apply tStep with (s:=S_First).
+ apply JO_red_dobind.
+ simpl; auto.
+ intros.
+ inversion H0.
+ substs.
+ apply red_not_value in H6; simpl in H6; intuition.
+ substs.
+ apply red_not_value in H6; simpl in H6; intuition.
+ substs.
+ intros.
+ inversion H0.
+ substs.
+  apply red_not_value in H1; simpl in H1; intuition.
+ inversion H0.
+ substs.
+ inversion H2.
+ substs.
+  apply red_not_value in H8; simpl in H8; intuition.
+ substs.
+ apply red_not_value in H2; simpl in H2; intuition.
+ apply red_not_value in H8; simpl in H8; intuition. 
+ reflexivity.
+ apply swapf_right.
+ simpl; auto.
+ simpl; auto.
+ substs.
+
+ exists s.
+ exists (
+      (LM_expr
+         ((E_taggingleft (E_taggingright (E_pair   (E_constant CONST_unit) (E_live_expr (LM_expr e)) )))))).
+ splits.
+ apply JO_red_forkdocomp1.
+ apply S_star with (y:= ( E_apply (swapf) (E_taggingleft (E_taggingright (E_pair  (E_constant CONST_unit) (E_live_expr (LM_expr e)) ))) )).
+ apply ttStep.
+ splits.
+ apply tStep with (s:=S_First).
+ apply JO_red_dobind.
+ simpl; auto.
+ intros.
+ inversion H0.
+ substs.
+ apply red_not_value in H6; simpl in H6; intuition.
+ substs.
+ apply red_not_value in H6; simpl in H6; intuition.
+ substs.
+ intros.
+ inversion H0.
+ substs.
+  apply red_not_value in H1; simpl in H1; intuition.
+ inversion H0.
+ substs.
+ inversion H2.
+ substs.
+  apply red_not_value in H8; simpl in H8; intuition.
+ substs.
+ apply red_not_value in H2; simpl in H2; intuition.
+ apply red_not_value in H8; simpl in H8; intuition. 
+ reflexivity.
+ apply swapf_left_right.
+ simpl; auto.
+ simpl; auto.
+ substs.
+
+ exists s.
+ exists (
+      (LM_expr
+         ((E_taggingleft (E_taggingleft (E_pair   (E_constant CONST_unit)  (E_constant CONST_unit) )))))).
+ splits.
+ apply JO_red_forkfincomp21.
+ apply S_star with (y:= ( E_apply (swapf) (E_taggingleft (E_taggingleft (E_pair   (E_constant CONST_unit)  (E_constant CONST_unit) ))) )).
+ apply ttStep.
+ splits.
+ apply tStep with (s:=S_First).
+ apply JO_red_dobind.
+ simpl; auto.
+ intros.
+ inversion H0.
+ substs.
+ apply red_not_value in H6; simpl in H6; intuition.
+ substs.
+ apply red_not_value in H6; simpl in H6; intuition.
+ substs.
+ intros.
+ inversion H0.
+ substs.
+  apply red_not_value in H1; simpl in H1; intuition.
+ inversion H0.
+ substs.
+ inversion H2.
+ substs.
+  apply red_not_value in H8; simpl in H8; intuition.
+ substs.
+ apply red_not_value in H2; simpl in H2; intuition.
+ apply red_not_value in H8; simpl in H8; intuition. 
+ reflexivity.
+ apply swapf_left_left.
+ simpl; auto.
+ simpl; auto.
+ substs.
+
+ exists s.
+ exists (
+      (LM_expr
+         ((E_taggingleft (E_taggingleft (E_pair   (E_constant CONST_unit)  (E_constant CONST_unit) )))))).
+ splits.
+ apply JO_red_forkfincomp12.
+ apply S_star with (y:= ( E_apply (swapf) (E_taggingleft (E_taggingleft (E_pair   (E_constant CONST_unit)  (E_constant CONST_unit) ))) )).
+ apply ttStep.
+ splits.
+ apply tStep with (s:=S_First).
+ apply JO_red_dobind.
+ simpl; auto.
+ intros.
+ inversion H0.
+ substs.
+ apply red_not_value in H6; simpl in H6; intuition.
+ substs.
+ apply red_not_value in H6; simpl in H6; intuition.
+ substs.
+ intros.
+ inversion H0.
+ substs.
+  apply red_not_value in H1; simpl in H1; intuition.
+ inversion H0.
+ substs.
+ inversion H2.
+ substs.
+  apply red_not_value in H8; simpl in H8; intuition.
+ substs.
+ apply red_not_value in H2; simpl in H2; intuition.
+ apply red_not_value in H8; simpl in H8; intuition. 
+ reflexivity.
+ apply swapf_left_left.
+ simpl; auto.
+ simpl; auto.
+Qed.
+ 
+
+Lemma fork_comm_tau_fin_h : forall (x y : expr), tauRed x y ->  ((fun x y => (exists ( p q lm : livemodes ), x = ((E_apply(E_apply (E_constant CONST_fork) (E_live_expr (p))) (E_live_expr (q)))) /\ y = (E_live_expr lm) ) ->
+               (exists ( p q lm lm': livemodes ), x = ((E_apply(E_apply (E_constant CONST_fork) (E_live_expr (p))) (E_live_expr (q)))) /\ y = (E_live_expr lm) /\ tauRed (((E_apply(E_apply (E_constant CONST_fork) (E_live_expr (q))) (E_live_expr (p)))) >>= swapf) (E_live_expr lm) /\  tauRed (((E_apply(E_apply (E_constant CONST_fork) (E_live_expr (q))) (E_live_expr (p))))) (E_live_expr lm') /\ totalTauRed ((E_live_expr lm') >>= swapf) ((E_live_expr lm)))) x y).
+Proof.
+ apply star_ind.
+ intros.
+ destruct H; destruct H; destruct H.
+ intuition.
+ rewrite -> H1 in H0.
+ discriminate H0.
+ intros.
+ destruct H2; destruct H2; destruct H2.
+ intuition.
+ substs.
+ 
+ inversion H.
+ substs.
+ inversion H2.
+ substs.
+ 
+ assert (exists p q lm lm',
+     E_apply (E_apply (E_constant CONST_fork) (E_live_expr (LM_expr e'')))
+       (E_live_expr (LM_expr e')) =
+     E_apply (E_apply (E_constant CONST_fork) (E_live_expr p))
+       (E_live_expr q) /\
+     E_live_expr x2 = E_live_expr lm /\
+     tauRed
+       (E_apply (E_apply (E_constant CONST_fork) (E_live_expr q))
+          (E_live_expr p) >>= swapf) (E_live_expr lm) /\
+     tauRed
+       (E_apply (E_apply (E_constant CONST_fork) (E_live_expr q))
+          (E_live_expr p)) (E_live_expr lm') /\
+     totalTauRed (E_live_expr lm' >>= swapf) (E_live_expr lm)).
+
+
+
+ apply H1.
+ exists (LM_expr e'') (LM_expr e') x2; splits; [reflexivity | reflexivity ].
+ destruct H3; destruct H3; destruct H3; destruct H3; intuition.
+  simplify_eq H4; simplify_eq H3; intros; substs; clear H3; clear H4.
+ exists (LM_expr e) (LM_expr e') x1 x3.
+   splits.
+ reflexivity.
+ reflexivity.
+
+ apply S_star with (y:=((E_apply (E_apply (E_constant CONST_fork) (E_live_expr (LM_expr e')))
+          (E_live_expr (LM_expr e''))) >>= swapf )).
+ apply tStep with (s:=S_Second).
+ apply JO_red_evalbind.
+ apply JO_red_forkmove2 with (s:=s0).
+ assumption.
+ assumption.
+ assumption.
+ apply S_star with (y:=((E_apply (E_apply (E_constant CONST_fork) (E_live_expr (LM_expr e')))
+          (E_live_expr (LM_expr e''))))).
+ apply tStep with (s:=S_Second).
+ apply JO_red_forkmove2 with (s:=s0).
+ assumption.
+ assumption.
+ assumption.
+ assumption.
+ substs.
+
+ assert ( exists p q lm lm',
+     E_apply (E_apply (E_constant CONST_fork) (E_live_expr (LM_expr e)))
+       (E_live_expr (LM_expr e'')) =
+     E_apply (E_apply (E_constant CONST_fork) (E_live_expr p))
+       (E_live_expr q) /\
+     E_live_expr x2 = E_live_expr lm /\
+     tauRed
+       (E_apply (E_apply (E_constant CONST_fork) (E_live_expr q))
+          (E_live_expr p) >>= swapf) (E_live_expr lm) /\
+     tauRed
+       (E_apply (E_apply (E_constant CONST_fork) (E_live_expr q))
+          (E_live_expr p)) (E_live_expr lm') /\
+     totalTauRed (E_live_expr lm' >>= swapf) (E_live_expr lm)).
+ apply H1.
+ exists (LM_expr e) (LM_expr e'') x2.
+ splits; [reflexivity | reflexivity].
+ destruct H3; destruct H3; destruct H3; destruct H3; intuition.
+ simplify_eq H4; simplify_eq H3; intros; substs.
+ clear H3; clear H4.
+ exists (LM_expr e) (LM_expr e') x1 x3.
+   splits.
+ reflexivity.
+ reflexivity.
+ apply S_star with (y:=((E_apply (E_apply (E_constant CONST_fork) (E_live_expr (LM_expr e'')))
+          (E_live_expr (LM_expr e))) >>= swapf )).
+ apply tStep with (s:=S_First).
+ apply JO_red_evalbind.
+ apply JO_red_forkmove1 with (s:=s0).
+ assumption.
+ assumption.
+ assumption.
+ apply S_star with (y:=((E_apply (E_apply (E_constant CONST_fork) (E_live_expr (LM_expr e'')))
+          (E_live_expr (LM_expr e))))).
+ apply tStep with (s:=S_First).
+ apply JO_red_forkmove1 with (s:=s0).
+ assumption.
+ assumption.
+ assumption.
+ assumption.
+ substs.
+ apply taured_val_id in H0.
+ apply fork_comm_step_fin in H2.
+ destruct H2.
+ destruct H2; intuition.
+ 
+ exists (LM_expr v) (LM_expr e) x2 x0.
+ splits.
+ reflexivity.
+ reflexivity.
+ apply S_star with (y:=((E_live_expr x0) >>= swapf)).
+ apply tStep with (s:=x).
+ apply JO_red_evalbind with (s:=x).
+ assumption.
+ apply tau_incl_totalTau.
+ simplify_eq H0; clear H0; intros; substs.
+ assumption.
+ apply S_star with (y:=((E_live_expr x0))).
+ apply tStep with (s:=x).
+ assumption.
+ apply star_refl.
+ substs.
+  simplify_eq H0; clear H0; intros; substs.
+ assumption.
+ simpl; auto.
+ substs.
+
+ apply taured_val_id in H0.
+ apply fork_comm_step_fin in H2.
+ destruct H2.
+ destruct H2; intuition.
+ 
+  exists (LM_expr e) (LM_expr v') x2 x0.
+ splits.
+ reflexivity.
+ reflexivity.
+ apply S_star with (y:=((E_live_expr x0) >>= swapf)).
+ apply tStep with (s:=x).
+ apply JO_red_evalbind with (s:=x).
+ assumption.
+ apply tau_incl_totalTau.
+ simplify_eq H0; intros; substs.
+ assumption.
+ apply S_star with (y:=((E_live_expr x0))).
+ apply tStep with (s:=x).
+ assumption.
+ apply star_refl.
+ simplify_eq H0; intros; substs.
+ assumption.
+ simpl; auto.
+ substs.
+
+ apply taured_val_id in H0.
+ apply fork_comm_step_fin in H2.
+ destruct H2.
+ destruct H2; intuition.
+ 
+ exists (LM_expr v) (LM_expr v') x2 x0.
+ splits.
+ reflexivity.
+ reflexivity.
+ apply S_star with (y:=((E_live_expr x0) >>= swapf)).
+ apply tStep with (s:=x).
+ apply JO_red_evalbind with (s:=x).
+ assumption.
+ apply tau_incl_totalTau.
+ simplify_eq H0; intros; substs.
+ assumption.
+ apply S_star with (y:=((E_live_expr x0))).
+ apply tStep with (s:=x).
+ assumption.
+ apply star_refl.
+ simplify_eq H0; intros; substs.
+ assumption.
+ simpl; auto.
+ substs.
+ 
+ apply red_not_value in H8; simpl in H8; intuition.
+ apply red_not_value in H9; simpl in H9; intuition.
+Qed.
+
+               
+Lemma fork_comm_tau_fin : forall ( p q lm : livemodes ), tauRed ((E_apply(E_apply (E_constant CONST_fork) (E_live_expr (p))) (E_live_expr (q)))) (E_live_expr lm) -> 
+                                                          tauRed (((E_apply (E_apply (E_constant CONST_fork) (E_live_expr (q))) (E_live_expr (p)))) >>= swapf) (E_live_expr lm) /\
+                                                          (exists (lm' : livemodes), tauRed (((E_apply (E_apply (E_constant CONST_fork) (E_live_expr (q))) (E_live_expr (p))))) (E_live_expr lm') /\ totalTauRed ((E_live_expr lm')>>= swapf)(E_live_expr lm) ).
+Proof.
+ intros.
+ apply fork_comm_tau_fin_h in H.
+ destruct H; destruct H; destruct H; destruct H.
+ intuition.
+ simplify_eq H0; simplify_eq H; intros; substs; clear H0; clear H.
+ assumption.
+ exists x2.
+  simplify_eq H0; simplify_eq H; intros; substs; clear H0; clear H.
+ splits.
+ assumption.
+ assumption.
+ exists p q lm; splits; [ reflexivity | reflexivity ].
+Qed.
+
+Lemma bind_tau_behave_back_h : forall (x y : expr), tauRed x y -> ((fun x y => (exists (e e' : expr), x = (e >>= e') ) -> (exists (e e' : expr), x = (e >>= e') /\ ((exists (f : expr), tauRed e f /\ y = (f >>= e')) \/ (exists (f : expr), tauRed e (E_live_expr (LM_expr f)) /\ ((exists (f' : expr ), (tauRed f f' /\ y=(((E_live_expr (LM_expr f')))>>=e') ) \/ (tauRed f f' /\ is_value_of_expr f' /\ tauRed (E_apply e' f') y))))) )   ) x y). 
+Proof.
+ apply star_ind.
+ intros.
+ destruct H; destruct H.
+ substs.
+ exists x0 x1.
+ splits.
+ reflexivity.
+ left.
+ exists x0.
+ splits.
+ apply star_refl.
+ reflexivity.
+ intros.
+ destruct H2; destruct H2; substs.
+ exists x0 x1.
+ splits.
+ reflexivity.
+ inversion H.
+ substs.
+ inversion H2.
+ substs.
+ assert (  exists e e'0,
+     e' >>= x1 = e >>= e'0 /\
+     ((exists f, tauRed e f /\ z = f >>= e'0) \/
+      (exists f,
+       tauRed e (E_live_expr (LM_expr f)) /\
+       (exists f',
+        tauRed f f' /\ z = E_live_expr (LM_expr f') >>= e'0 \/
+        tauRed f f' /\ is_value_of_expr f' /\ tauRed (E_apply e'0 f') z)))).
+ apply H1.
+ exists e' x1.
+ reflexivity.
+ destruct H3; destruct H3.
+ intuition.
+ simplify_eq H4; clear H4; intros; substs.
+ destruct H3.
+ intuition.
+ substs.
+ left.
+ exists x1.
+ splits.
+ apply S_star with (y:=x).
+ apply tStep with (s:=s).
+ assumption.
+ assumption.
+ reflexivity.
+ simplify_eq H4; clear H4; intros; substs.
+ right.
+ destruct H3.
+ exists x1.
+ splits.
+ apply S_star with (y:=x).
+ apply tStep with (s:=s).
+ assumption.
+ intuition.
+ intuition.
+ substs.
+ assert ( exists e e'0,
+     E_live_expr (LM_expr e') >>= x1 = e >>= e'0 /\
+     ((exists f, tauRed e f /\ z = f >>= e'0) \/
+      (exists f,
+       tauRed e (E_live_expr (LM_expr f)) /\
+       (exists f',
+        tauRed f f' /\ z = E_live_expr (LM_expr f') >>= e'0 \/
+        tauRed f f' /\ is_value_of_expr f' /\ tauRed (E_apply e'0 f') z)))).
+ apply H1.
+ exists (E_live_expr (LM_expr e')) (x1).
+ reflexivity.
+ destruct H3; destruct H3.
+ intuition.
+ substs.
+ simplify_eq H4; clear H4; intros; substs.
+ destruct H3; elim H3; intros.
+ simplify_eq H5; clear H5; intros; substs.
+ apply taured_val_id in H4.
+ substs.
+ right.
+ exists e.
+ splits.
+ apply star_refl.
+ 
+ exists e'.
+ left.
+ splits.
+ apply S_star with (y:=e').
+ apply tStep with (s:=s).
+ assumption.
+ apply star_refl.
+ apply reflexivity.
+ simpl; auto.
+ simplify_eq H4; clear H4; intros; substs.
+ destruct H3.
+ elim H3.
+ intros.
+ apply taured_val_id in H4.
+ simplify_eq H4; clear H4; intros; substs.
+ destruct H5.
+ destruct H4.
+ clear H3.
+ intuition.
+ substs.
+ right.
+ exists e.
+ splits.
+ apply star_refl.
+ exists x1.
+ left.
+ splits.
+ apply S_star with (y:=x).
+ apply tStep with (s:=s).
+ assumption.
+ assumption.
+ apply reflexivity.
+ clear H3.
+ intuition.
+ right.
+ exists e.
+ splits.
+ apply star_refl.
+ exists x1.
+ right.
+ splits.
+ apply S_star with (y:=x).
+ apply tStep with (s:=s).
+ assumption.
+ assumption.
+ assumption.
+ assumption.
+ simpl; auto.
+ substs.
+ right.
+ exists v.
+ splits.
+ apply star_refl.
+ exists v.
+ right.
+ splits.
+ apply star_refl.
+ assumption.
+ assumption.
+Qed.
+
+
+
+Lemma fork_swap_tau_behave : forall (e : expr )( p q : livemodes ), tauRed (E_bind (E_apply (E_apply (E_constant CONST_fork) (E_live_expr (p))) (E_live_expr (q))) (swapf)) e ->
+                                 ((exists (p' q' : livemodes), e = (E_bind (E_apply (E_apply (E_constant CONST_fork) (E_live_expr (p'))) (E_live_expr (q'))) (swapf)) /\ tauRed (E_apply (E_apply (E_constant CONST_fork) (E_live_expr (p))) (E_live_expr (q)))  (E_apply (E_apply (E_constant CONST_fork) (E_live_expr (p'))) (E_live_expr (q'))) ) \/ 
+                                 ((exists (lm : livemodes),  tauRed ( (E_apply (E_apply (E_constant CONST_fork) (E_live_expr (p))) (E_live_expr (q)))) (E_live_expr lm) /\ totalTauRed ((E_live_expr lm) >>= swapf) e)) ).
+Proof.
+ intros.
+ assert (H0:=H).
+ apply bind_tau_behave_back_h in H0. 
+ destruct H0.
+ destruct H0.
+ intuition.
+ simplify_eq H1; clear H1; intros; substs.
+ destruct H0.
+ intuition.
+ assert (K:=H1).
+ simplify_eq H2; clear H2; intros; substs.
+ induction p; induction q.
+ apply fork_tau_behave_cc in H1.
+ substs.
+ left.
+ exists (LM_comp lab) (LM_comp lab0).
+ splits; [reflexivity | apply star_refl].
+ apply fork_tau_behave_ce in H1.
+ substs.
+ left.
+ exists (LM_comp lab) (LM_expr expr5).
+ splits; [reflexivity | apply star_refl].
+ apply fork_tau_behave_ec in H1.
+ substs.
+ left.
+ exists (LM_expr expr5) (LM_comp lab).
+ splits; [reflexivity | apply star_refl].
+ assert (L:=H1).
+ apply fork_tau_behave_ee in H1.
+ intuition.
+ destruct H0; destruct H0; intuition; substs.
+ left.
+ exists (LM_expr x0) (LM_expr x1).
+ splits; [reflexivity | assumption].
+ destruct H1; destruct H0; intuition; substs.
+ right.
+ exists ((LM_expr (E_taggingright (E_pair (E_live_expr (LM_expr x0)) x1)))).
+ splits.
+ assumption.
+ apply star_refl.
+ destruct H0; destruct H0; intuition; substs.
+ right.
+ exists ((LM_expr (E_taggingleft (E_taggingleft (E_pair x0 x1))))).
+ splits.
+ assumption.
+ apply star_refl.
+ destruct H0; destruct H0; intuition; substs.
+ right.
+ exists ((LM_expr
+            (E_taggingleft
+               (E_taggingright (E_pair x0 (E_live_expr (LM_expr x1))))))).
+ splits.
+ assumption.
+ apply star_refl.
+ destruct H0.
+ intuition.
+ destruct H3.
+ intuition.
+ substs.
+ simplify_eq H1; clear H1; intros; substs.
+ right.
+ exists (LM_expr x1).
+ splits.
+ assumption.
+ induction p; induction q.
+ apply fork_tau_behave_cc in H2.
+ discriminate H2.
+ apply fork_tau_behave_ce in H2.
+ discriminate H2.
+ apply fork_tau_behave_ec in H2.
+ discriminate H2.
+ assert (L:=H2).
+ apply fork_tau_behave_ee in H2.
+ intuition.
+ destruct H1; destruct H1; intuition.
+ discriminate H4.
+ destruct H2; destruct H1; intuition.
+ simplify_eq H5; clear H5; intros; substs.
+ apply taured_val_id in H0.
+ substs.
+ apply star_refl.
+ simpl.
+ auto.
+ destruct H1; destruct H1; intuition.
+ simplify_eq H6; clear H6; intros; substs.
+ apply taured_val_id in H0.
+ substs.
+ apply star_refl.
+ simpl.
+ auto.
+ destruct H1; destruct H1; intuition.
+ simplify_eq H5; clear H5; intros; substs.
+ apply taured_val_id in H0.
+ substs.
+ apply star_refl.
+ simpl.
+ auto.
+ simplify_eq H1; clear H1; intros; substs.
+ right.
+ exists (LM_expr x1).
+ induction p; induction q.
+ apply fork_tau_behave_cc in H2.
+ discriminate H2.
+ apply fork_tau_behave_ce in H2.
+ discriminate H2.
+ apply fork_tau_behave_ec in H2.
+ discriminate H2.
+ assert (L:=H2).
+ apply fork_tau_behave_ee in H2.
+ intuition.
+ destruct H1; destruct H1; intuition.
+ discriminate H6.
+ destruct H2; destruct H1; intuition.
+ simplify_eq H7; clear H7; intros; substs.
+ apply taured_val_id in H0.
+ substs.
+ assert (totalTauRed (E_apply swapf (E_taggingright (E_pair (E_live_expr (LM_expr x)) x0)))
+    (E_live_expr
+       (LM_expr (E_taggingleft (E_taggingright (E_pair x0 (E_live_expr (LM_expr x)))))))).
+ apply swapf_right.
+ simpl; auto.
+ assumption.
+ assert (totalTauRed
+       (E_apply swapf (E_taggingright (E_pair (E_live_expr (LM_expr x)) x0)))
+       (E_live_expr
+          (LM_expr
+             (E_taggingleft
+                (E_taggingright (E_pair x0 (E_live_expr (LM_expr x))))))) /\ tauRed
+       (E_apply swapf (E_taggingright (E_pair (E_live_expr (LM_expr x)) x0)))
+       e).
+ splits; [assumption | assumption ].
+ apply ttau_prefix in H6.
+ intuition.
+ apply S_star with (y:=(E_apply swapf (E_taggingright (E_pair (E_live_expr (LM_expr x)) x0)))).
+ apply ttStep.
+ splits.
+ apply simpTau with (s:=S_First).
+ apply JO_red_dobind.
+ simpl; auto.
+ intros.
+ inversion H7.
+ apply red_not_value in H14; simpl in H14; intuition.
+ apply red_not_value in H14; simpl in H14; intuition.
+ intros.
+ inversion H7.
+ substs.
+ inversion H9.
+ substs.
+ apply red_not_value in H15; simpl in H15; intuition.
+ apply red_not_value in H15; simpl in H15; intuition.
+ apply reflexivity.
+ assumption.
+ apply taured_val_id in H7.
+ substs.
+ apply S_star with (y:=(E_apply swapf (E_taggingright (E_pair (E_live_expr (LM_expr x)) x0)))).
+ apply ttStep.
+ splits.
+ apply simpTau with (s:=S_First).
+ apply JO_red_dobind.
+ simpl; auto.
+ intros.
+ inversion H6.
+ apply red_not_value in H12; simpl in H12; intuition.
+ apply red_not_value in H12; simpl in H12; intuition.
+ intros.
+ inversion H6.
+ substs.
+ inversion H7.
+ substs.
+ apply red_not_value in H13; simpl in H13; intuition.
+ apply red_not_value in H13; simpl in H13; intuition.
+ apply reflexivity.
+ assumption.
+ apply taured_val_id in H7.
+ substs.
+ simpl; auto.
+ simpl; auto.
+ simpl; auto.
+
+
+destruct H1; destruct H1; intuition.
+ simplify_eq H8; clear H8; intros; substs.
+ apply taured_val_id in H0.
+ substs.
+ assert (totalTauRed
+       (E_apply swapf (E_taggingleft (E_taggingleft (E_pair x x0))))
+       (E_live_expr
+          (LM_expr
+             (E_taggingleft (E_taggingleft (E_pair x0 x))))) /\ tauRed (E_apply swapf (E_taggingleft (E_taggingleft (E_pair x x0)))) e).
+ splits.
+ apply swapf_left_left.
+ assumption.
+ assumption.
+ assumption.
+ apply ttau_prefix in H0.
+ intuition.
+ apply S_star with (y:=(E_apply swapf (E_taggingleft (E_taggingleft (E_pair x x0))))).
+ apply ttStep.
+ splits.
+ apply simpTau with (s:=S_First).
+ apply JO_red_dobind.
+ simpl; auto.
+ intros.
+ inversion H7.
+ apply red_not_value in H14; simpl in H14; intuition.
+ apply red_not_value in H14; simpl in H14; intuition.
+ intros.
+ inversion H7.
+ substs.
+ inversion H9.
+ substs.
+ apply red_not_value in H15; simpl in H15; intuition.
+ apply red_not_value in H15; simpl in H15; intuition.
+ apply reflexivity.
+ assumption.
+ apply taured_val_id in H7.
+ substs.
+ apply S_star with (y:=(E_apply swapf (E_taggingleft (E_taggingleft (E_pair x x0))))).
+ apply ttStep.
+ splits.
+ apply simpTau with (s:=S_First).
+ apply JO_red_dobind.
+ simpl; auto.
+ intros.
+ inversion H0.
+ apply red_not_value in H12; simpl in H12; intuition.
+ apply red_not_value in H12; simpl in H12; intuition.
+ intros.
+ inversion H0.
+ substs.
+ inversion H7.
+ substs.
+ apply red_not_value in H13; simpl in H13; intuition.
+ apply red_not_value in H13; simpl in H13; intuition.
+ apply reflexivity.
+ apply swapf_left_left. 
+assumption.
+ assumption.
+ simpl; auto.
+ simpl; auto.
+
+
+
+destruct H1; destruct H1; intuition.
+ simplify_eq H7; clear H7; intros; substs.
+ apply taured_val_id in H0.
+ substs.
+ assert (totalTauRed
+       (E_apply swapf
+          (E_taggingleft
+             (E_taggingright (E_pair x (E_live_expr (LM_expr x0))))))
+       (E_live_expr
+          (LM_expr
+             ( (E_taggingright (E_pair (E_live_expr (LM_expr x0)) x))))) /\ tauRed
+       (E_apply swapf
+          (E_taggingleft
+             (E_taggingright (E_pair x (E_live_expr (LM_expr x0)))))) e).
+ splits.
+ apply swapf_left_right.
+ assumption.
+ simpl; auto.
+ assumption.
+ apply ttau_prefix in H0.
+ intuition.
+ apply S_star with (y:=(E_apply swapf
+          (E_taggingleft
+             (E_taggingright (E_pair x (E_live_expr (LM_expr x0))))))).
+ apply ttStep.
+ splits.
+ apply simpTau with (s:=S_First).
+ apply JO_red_dobind.
+ simpl; auto.
+ intros.
+ inversion H6.
+ apply red_not_value in H13; simpl in H13; intuition.
+ apply red_not_value in H13; simpl in H13; intuition.
+ intros.
+ inversion H6.
+ substs.
+ inversion H8.
+ substs.
+ apply red_not_value in H14; simpl in H14; intuition.
+ apply red_not_value in H14; simpl in H14; intuition.
+ apply reflexivity.
+ assumption.
+ apply taured_val_id in H6.
+ substs.
+ apply S_star with (y:=(E_apply swapf
+          (E_taggingleft
+             (E_taggingright (E_pair x (E_live_expr (LM_expr x0))))))).
+ apply ttStep.
+ splits.
+ apply simpTau with (s:=S_First).
+ apply JO_red_dobind.
+ simpl; auto.
+ intros.
+ inversion H0.
+ apply red_not_value in H11; simpl in H11; intuition.
+ apply red_not_value in H11; simpl in H11; intuition.
+ intros.
+ inversion H0.
+ substs.
+ inversion H6.
+ substs.
+ apply red_not_value in H12; simpl in H12; intuition.
+ apply red_not_value in H12; simpl in H12; intuition.
+ apply reflexivity.
+ apply swapf_left_right. 
+assumption.
+ simpl; auto.
+ simpl; auto.
+ simpl; auto.
+
+
+ 
+ exists (E_apply (E_apply (E_constant CONST_fork) (E_live_expr p)) (E_live_expr q)) (swapf).
+ reflexivity.
+Qed.
+
+
+Lemma fork_swap_lab_behave : forall (e : expr )( p q : livemodes )(l : label), labRed l (E_bind (E_apply (E_apply (E_constant CONST_fork) (E_live_expr (p))) (E_live_expr (q))) (swapf)) e ->
+                                 ((exists (p' q' : livemodes), e = (E_bind (E_apply (E_apply (E_constant CONST_fork) (E_live_expr (p'))) (E_live_expr (q'))) (swapf)) /\ labRed l (E_apply (E_apply (E_constant CONST_fork) (E_live_expr (p))) (E_live_expr (q)))  (E_apply (E_apply (E_constant CONST_fork) (E_live_expr (p'))) (E_live_expr (q'))) ) \/ 
+                                 ((exists (lm : livemodes),  labRed l ( (E_apply (E_apply (E_constant CONST_fork) (E_live_expr (p))) (E_live_expr (q)))) (E_live_expr lm) /\ totalTauRed ((E_live_expr lm) >>= swapf) e)) ).
+Proof.
+ intros.
+ inversion H.
+ intuition; substs. 
+ assert (L:=H4).
+ apply fork_swap_tau_behave in H4.
+ intuition.
+ destruct H1; destruct H1.
+ intuition; substs.
+ inversion H0.
+ substs.
+ inversion H8.
+ substs.
+ assert (K:=H6).
+ apply fork_swap_tau_behave in H6.
+ intuition.
+ left.
+ destruct H1; destruct H1.
+ intuition; substs.
+ exists x x0.
+ splits.
+ reflexivity.
+ apply lab_r with (e1:=(E_apply (E_apply (E_constant CONST_fork) (E_live_expr (LM_expr e0)))
+          (E_live_expr (LM_expr e'0))))(e2:= E_apply (E_apply (E_constant CONST_fork) (E_live_expr (LM_expr e'')))
+       (E_live_expr (LM_expr e'0)))(s:=S_First).
+ splits; [assumption | assumption | assumption ].
+ destruct H1.
+ right.
+ exists x.
+ splits.
+ apply lab_r with (e1:=(E_apply (E_apply (E_constant CONST_fork) (E_live_expr (LM_expr e0)))
+       (E_live_expr (LM_expr e'0))))(e2:=(E_apply (E_apply (E_constant CONST_fork) (E_live_expr (LM_expr e'')))
+       (E_live_expr (LM_expr e'0))))(s:=S_First). splits.
+ assumption.
+ assumption.
+ intuition.
+ intuition.
+ substs. 
+
+  apply fork_swap_tau_behave in H6.
+ intuition.
+ left.
+ destruct H1; destruct H1.
+ intuition; substs.
+ exists x x0.
+ splits.
+ reflexivity.
+ apply lab_r with (e1:=(E_apply (E_apply (E_constant CONST_fork) (E_live_expr (LM_expr e0)))
+       (E_live_expr (LM_expr e'0))))(e2:= ( E_apply (E_apply (E_constant CONST_fork) (E_live_expr (LM_expr e0)))
+       (E_live_expr (LM_expr e''))))(s:=S_Second).
+ splits; [assumption | assumption | assumption ].
+ destruct H1.
+ right.
+ exists x.
+ splits.
+ apply lab_r with (e1:=(E_apply (E_apply (E_constant CONST_fork) (E_live_expr (LM_expr e0)))
+       (E_live_expr (LM_expr e'0))))(e2:=(E_apply (E_apply (E_constant CONST_fork) (E_live_expr (LM_expr e0)))
+       (E_live_expr (LM_expr e''))))(s:=S_Second). splits.
+ assumption.
+ assumption.
+ intuition.
+ intuition.
+ substs.
+
+ right.
+ exists  (LM_expr
+          (E_taggingleft
+             (E_taggingright
+                (E_pair (E_constant CONST_unit) (E_live_expr (LM_expr e0)))))).
+ splits.
+ apply lab_r with (e1:=( E_apply (E_apply (E_constant CONST_fork) (E_live_expr (LM_comp l)))
+       (E_live_expr (LM_expr e0))))(e2:=(E_live_expr
+       (LM_expr
+          (E_taggingleft
+             (E_taggingright
+                (E_pair (E_constant CONST_unit) (E_live_expr (LM_expr e0))))))))(s:=(s)).
+ splits.
+ assumption.
+ assumption.
+ apply star_refl.
+ assert ((totalTauRed (E_live_expr
+          (LM_expr
+             (E_taggingleft
+                (E_taggingright
+                   (E_pair (E_constant CONST_unit) (E_live_expr (LM_expr e0)))))) >>=
+        swapf) (E_live_expr
+          (LM_expr
+             (
+                (E_taggingright
+                   (E_pair  (E_live_expr (LM_expr e0)) (E_constant CONST_unit))))) )) /\ (tauRed
+       (E_live_expr
+          (LM_expr
+             (E_taggingleft
+                (E_taggingright
+                   (E_pair (E_constant CONST_unit) (E_live_expr (LM_expr e0)))))) >>=
+        swapf) e)).
+ splits.
+ apply swapf_left_right_b.
+ simpl; auto.
+ simpl; auto.
+ assumption.
+ apply ttau_prefix in H1.
+ intuition.
+ apply taured_val_id in H2.
+ substs.
+ apply swapf_left_right_b.
+ simpl; auto.
+ simpl; auto.
+ simpl; auto.
+ substs.
+ right.
+ exists ((LM_expr
+          (E_taggingright
+             (E_pair (E_live_expr (LM_expr e0)) (E_constant CONST_unit))))).
+ splits.
+ apply lab_r with (e1:=(E_apply (E_apply (E_constant CONST_fork) (E_live_expr (LM_expr e0)))
+       (E_live_expr (LM_comp l))))(e2:=( E_live_expr
+       (LM_expr
+          (E_taggingright
+             (E_pair (E_live_expr (LM_expr e0)) (E_constant CONST_unit))))))(s:=s). splits.
+ assumption.
+ assumption.
+ apply star_refl.
+ assert ((totalTauRed
+       (E_live_expr
+          (LM_expr
+             (E_taggingright
+                (E_pair (E_live_expr (LM_expr e0)) (E_constant CONST_unit)))) >>=
+        swapf) (E_live_expr
+          (LM_expr
+            (E_taggingleft
+             (E_taggingright
+                (E_pair  (E_constant CONST_unit) (E_live_expr (LM_expr e0)))))) )) /\ (tauRed
+       (E_live_expr
+          (LM_expr
+             (E_taggingright
+                (E_pair (E_live_expr (LM_expr e0)) (E_constant CONST_unit)))) >>=
+        swapf) e)).
+ splits.
+ apply swapf_right_b.
+ simpl; auto.
+ simpl; auto.
+ assumption.
+ apply ttau_prefix in H1.
+ intuition.
+ apply taured_val_id in H2; substs.
+ apply swapf_right_b.
+ simpl; auto.
+ simpl; auto.
+ simpl; auto.
+ substs.
+ apply fork_swap_tau_behave in H6.
+ intuition.
+ left.
+ destruct H1; destruct H1.
+ intuition; substs.
+ exists x x0.
+ splits.
+ reflexivity.
+ apply lab_r with (e1:=(E_apply (E_apply (E_constant CONST_fork) (E_live_expr (LM_comp l)))
+       (E_live_expr (LM_comp label''))))(e2:=(E_apply
+       (E_apply (E_constant CONST_fork)
+          (E_live_expr (LM_expr (E_constant CONST_unit))))
+       (E_live_expr (LM_comp label''))))(s:=S_First).
+ splits.
+ assumption.
+ assumption.
+ assumption.
+ right.
+ destruct H1; intuition.
+ exists x.
+ splits.
+ apply fork_tau_behave_ec in H2.
+ discriminate H2.
+ apply fork_tau_behave_ec in H2.
+ discriminate H2.
+ substs.
+ apply fork_swap_tau_behave in H6.
+ intuition.
+ left.
+ destruct H1; destruct H1.
+ intuition; substs.
+ exists x x0.
+ splits.
+ reflexivity.
+ apply lab_r with (e1:=(E_apply (E_apply (E_constant CONST_fork) (E_live_expr (LM_comp label5)))
+       (E_live_expr (LM_comp l))))(e2:=(E_apply (E_apply (E_constant CONST_fork) (E_live_expr (LM_comp label5)))
+       (E_live_expr (LM_expr (E_constant CONST_unit)))))(s:=S_Second).
+ splits.
+ assumption.
+ assumption.
+ assumption.
+ right.
+ destruct H1; intuition.
+ exists x.
+ splits.
+ apply fork_tau_behave_ce in H2.
+ discriminate H2.
+ apply fork_tau_behave_ce in H2.
+ discriminate H2.
+ substs.
+ right.
+ exists ((LM_expr
+          (E_taggingleft
+             (E_taggingleft
+                (E_pair (E_constant CONST_unit) (E_constant CONST_unit)))))).
+ splits.
+ apply lab_r with (e1:=(E_apply
+       (E_apply (E_constant CONST_fork)
+          (E_live_expr (LM_expr (E_constant CONST_unit))))
+       (E_live_expr (LM_comp l))))(e2:=( E_live_expr
+       (LM_expr
+          (E_taggingleft
+             (E_taggingleft
+                (E_pair (E_constant CONST_unit) (E_constant CONST_unit)))))))(s:=s).
+ splits.
+ assumption.
+ assumption.
+ apply star_refl.
+ assert ((totalTauRed
+       (E_live_expr
+          (LM_expr
+             (E_taggingleft
+                (E_taggingleft
+                   (E_pair (E_constant CONST_unit) (E_constant CONST_unit))))) >>=
+        swapf) (E_live_expr
+          (LM_expr
+             (E_taggingleft
+                (E_taggingleft
+                   (E_pair (E_constant CONST_unit) (E_constant CONST_unit))))))) /\ (tauRed
+       (E_live_expr
+          (LM_expr
+             (E_taggingleft
+                (E_taggingleft
+                   (E_pair (E_constant CONST_unit) (E_constant CONST_unit))))) >>=
+        swapf) e)).
+ splits.
+ apply swapf_left_left_b.
+ simpl; auto.
+ simpl; auto.
+ assumption.
+ apply ttau_prefix in H1.
+ intuition.
+ apply taured_val_id in H2.
+ substs.
+ apply swapf_left_left_b.
+ simpl; auto.
+ simpl; auto.
+ simpl; auto.
+ substs.
+
+ right.
+ exists ((LM_expr
+          (E_taggingleft
+             (E_taggingleft
+                (E_pair (E_constant CONST_unit) (E_constant CONST_unit)))))).
+ splits.
+ apply lab_r with (e1:=(E_apply
+       (E_apply (E_constant CONST_fork)
+          (E_live_expr (LM_comp l)))
+       (E_live_expr (LM_expr (E_constant CONST_unit)))))(e2:=( E_live_expr
+       (LM_expr
+          (E_taggingleft
+             (E_taggingleft
+                (E_pair (E_constant CONST_unit) (E_constant CONST_unit)))))))(s:=s).
+ splits.
+ assumption.
+ assumption.
+ apply star_refl.
+ assert ((totalTauRed
+       (E_live_expr
+          (LM_expr
+             (E_taggingleft
+                (E_taggingleft
+                   (E_pair (E_constant CONST_unit) (E_constant CONST_unit))))) >>=
+        swapf) (E_live_expr
+          (LM_expr
+             (E_taggingleft
+                (E_taggingleft
+                   (E_pair (E_constant CONST_unit) (E_constant CONST_unit))))))) /\ (tauRed
+       (E_live_expr
+          (LM_expr
+             (E_taggingleft
+                (E_taggingleft
+                   (E_pair (E_constant CONST_unit) (E_constant CONST_unit))))) >>=
+        swapf) e)).
+ splits.
+ apply swapf_left_left_b.
+ simpl; auto.
+ simpl; auto.
+ assumption.
+ apply ttau_prefix in H1.
+ intuition.
+ apply taured_val_id in H2.
+ substs.
+ apply swapf_left_left_b.
+ simpl; auto.
+ simpl; auto.
+ simpl; auto.
+ substs.
+ apply red_not_value in H9; simpl in H9; intuition.
+ apply red_not_value in H10; simpl in H10; intuition.
+ destruct H1.
+ intuition.
+ induction p; induction q.
+ apply fork_tau_behave_cc in H2; discriminate H2.
+  apply fork_tau_behave_ce in H2; discriminate H2.
+ apply fork_tau_behave_ec in H2; discriminate H2.
+  apply fork_tau_behave_ee in H2.
+ intuition.
+ destruct H1.
+ destruct H1.
+ intuition.
+ discriminate H5.
+ destruct H2; destruct H1; intuition.
+ simplify_eq H7; clear H7; intros; substs.
+ assert ((totalTauRed
+        (E_live_expr
+          (LM_expr (E_taggingright (E_pair (E_live_expr (LM_expr x0)) x1))) >>=
+        swapf) (E_live_expr
+          (LM_expr
+             (E_taggingleft
+                (E_taggingright
+                   (E_pair x1 (E_live_expr (LM_expr x0)))))))) /\ (tauRed
+       (E_live_expr
+          (LM_expr (E_taggingright (E_pair (E_live_expr (LM_expr x0)) x1))) >>=
+        swapf) e1)).
+ splits.
+ apply swapf_right_b.
+ simpl; auto.
+ assumption.
+ apply tau_incl_totalTau.
+ assumption.
+ apply ttau_prefix in H5.
+ intuition.
+ inversion H8.
+ substs.
+ inversion H0.
+ substs.
+ inversion H7.
+ substs.
+ intuition.
+ apply H10 in H0.
+ intuition.
+ apply taured_val_id in H7.
+ substs.
+ inversion H0.
+ simpl; auto.
+
+ destruct H1; destruct H1; intuition.
+ simplify_eq H8; clear H8; intros; substs.
+ assert ((totalTauRed
+        (E_live_expr (LM_expr (E_taggingleft (E_taggingleft (E_pair x0 x1)))) >>=
+        swapf) (E_live_expr
+          (LM_expr
+             (E_taggingleft
+                (E_taggingleft
+                   (E_pair x1 x0)))))) /\ (tauRed
+       (E_live_expr (LM_expr (E_taggingleft (E_taggingleft (E_pair x0 x1)))) >>=
+        swapf) e1)).
+ splits.
+ apply swapf_left_left_b.
+ simpl; auto.
+ assumption.
+ apply tau_incl_totalTau.
+ assumption.
+ apply ttau_prefix in H7.
+ intuition.
+ inversion H9.
+ substs.
+ apply red_not_value in H0; simpl in H0; intuition.
+ substs.
+ inversion H8.
+ intuition.
+ apply H11 in H0.
+ intuition.
+
+
+ assert ((totalTauRed
+        (E_live_expr (LM_expr (E_taggingleft (E_taggingleft (E_pair x0 x1)))) >>=
+        swapf) (E_live_expr
+          (LM_expr
+             (E_taggingleft
+                (E_taggingleft
+                   (E_pair x1 x0)))))) /\ (tauRed
+       (E_live_expr (LM_expr (E_taggingleft (E_taggingleft (E_pair x0 x1)))) >>=
+        swapf) e1)).
+ splits.
+ apply swapf_left_left_b.
+ simpl; auto.
+ assumption.
+ apply tau_incl_totalTau.
+ assumption.
+ apply ttau_prefix in H7.
+ intuition.
+ inversion H10.
+ substs.
+ apply red_not_value in H0; simpl in H0; intuition.
+ substs.
+ inversion H9.
+ intuition.
+ apply H12 in H0.
+ intuition.
+ apply taured_val_id in H8; substs.
+ apply red_not_value in H0; simpl in H0; intuition.
+ simpl; auto.
+
+ destruct H1; destruct H1; intuition.
+ simplify_eq H7; clear H7; intros; substs.
+ assert ((totalTauRed
+        (E_live_expr
+          (LM_expr
+             (E_taggingleft
+                (E_taggingright (E_pair x0 (E_live_expr (LM_expr x1)))))) >>=
+        swapf) (E_live_expr
+          (LM_expr
+             (
+                (E_taggingright (E_pair (E_live_expr (LM_expr x1)) x0 )))))) /\ (tauRed
+       (E_live_expr
+          (LM_expr
+             (E_taggingleft
+                (E_taggingright (E_pair x0 (E_live_expr (LM_expr x1)))))) >>=
+        swapf) e1)).
+ splits.
+ apply swapf_left_right_b.
+ simpl; auto.
+ simpl; auto.
+ apply tau_incl_totalTau.
+ assumption.
+ apply ttau_prefix in H5.
+ intuition.
+ inversion H8.
+ substs.
+ apply red_not_value in H0; simpl in H0; intuition.
+ substs.
+ inversion H7.
+ intuition.
+ apply H10 in H0.
+ intuition.
+ apply taured_val_id in H7.
+ substs.
+ apply red_not_value in H0; simpl in H0; intuition.
+ simpl; auto.
+Qed.
+
+
+Lemma ttr_val_not_labred : forall (e v e' : expr)(l:label), totalTauRed e v /\ is_value_of_expr v -> (~ (labRed l e e')).
+Proof.
+ intros.
+ intuition.
+ inversion H0.
+ intuition.
+ assert (totalTauRed e v /\ tauRed e e1).
+ auto.
+ apply ttau_prefix in H7.
+ intuition.
+ inversion H10.
+ substs.
+ apply red_not_value in H; contradiction.
+ substs.
+ inversion H9.
+ intuition.
+ apply H3 in H.
+ auto.
+ substs.
+ inversion H9.
+ substs.
+ apply red_not_value in H; contradiction.
+ substs.
+ inversion H3.
+ apply red_not_value in H5; contradiction.
+Qed.
+
+Lemma fork_comm_taured_ee_laststep_h : forall (x y : expr), tauRed x y -> ((fun x y => 
+   ( exists ( e e' : expr) (lm : livemodes),  
+       x = (E_apply
+         (E_apply (E_constant CONST_fork) (E_live_expr (LM_expr e')))
+         (E_live_expr (LM_expr e))) /\
+       y = (E_live_expr  lm)) -> 
+( exists (e e' : expr) (lm : livemodes), 
+       x = (E_apply
+         (E_apply (E_constant CONST_fork) (E_live_expr (LM_expr e')))
+         (E_live_expr (LM_expr e))) /\ 
+       y = (E_live_expr  lm) /\
+       (exists (p q : expr), tauRed x (E_apply
+         (E_apply (E_constant CONST_fork) (E_live_expr (LM_expr q)))
+         (E_live_expr (LM_expr p))) /\ tauStep (E_apply
+         (E_apply (E_constant CONST_fork) (E_live_expr (LM_expr q)))
+         (E_live_expr (LM_expr p))) (E_live_expr  lm) )))x y ).
+Proof.
+ apply star_ind.
+ intros.
+ destruct H; destruct H; destruct H; destruct H; intuition; substs.
+ discriminate H0.
+ intros.
+ destruct H2; destruct H2; destruct H2; destruct H2; intuition; substs.
+ exists x0 x1 x2.
+ splits.
+ reflexivity.
+ reflexivity.
+ assert  (tauRed
+      (E_apply (E_apply (E_constant CONST_fork) (E_live_expr (LM_expr x1)))
+         (E_live_expr (LM_expr x0))) y).
+ apply S_star with (y:=y).
+ assumption.
+ apply star_refl.
+ apply fork_tau_behave_ee in H2.
+ intuition.
+ destruct H3. destruct H2.
+ intuition. 
+ substs.
+ assert (exists e e' lm,
+     E_apply (E_apply (E_constant CONST_fork) (E_live_expr (LM_expr x)))
+       (E_live_expr (LM_expr x3)) =
+     E_apply (E_apply (E_constant CONST_fork) (E_live_expr (LM_expr e')))
+       (E_live_expr (LM_expr e)) /\
+     E_live_expr x2 = E_live_expr lm /\
+     (exists p q,
+      tauRed
+        (E_apply (E_apply (E_constant CONST_fork) (E_live_expr (LM_expr x)))
+           (E_live_expr (LM_expr x3)))
+        (E_apply (E_apply (E_constant CONST_fork) (E_live_expr (LM_expr q)))
+           (E_live_expr (LM_expr p))) /\
+      tauStep
+        (E_apply (E_apply (E_constant CONST_fork) (E_live_expr (LM_expr q)))
+           (E_live_expr (LM_expr p))) (E_live_expr lm))).
+ apply H1.
+ exists x3 x x2.
+ splits.
+ reflexivity.
+ reflexivity.
+ destruct H4. destruct H4. destruct H4. intuition.
+ simplify_eq H5; simplify_eq H4; clear H5; clear H4; intros; substs.
+ destruct H7. destruct H4. intuition.
+ exists x x2.
+ splits.
+ apply S_star with  (y:=(E_apply (E_apply (E_constant CONST_fork) (E_live_expr (LM_expr x5)))
+          (E_live_expr (LM_expr x4)))).
+ assumption.
+ assumption.
+ assumption.
+ exists x0 x1.
+ destruct H2. destruct H2.
+ intuition.
+ substs.
+ apply star_refl.
+ substs.
+ apply taured_val_id in H0.
+ simplify_eq H0; clear H0; intros; substs.
+ assumption.
+ simpl; auto.
+ exists x0 x1.
+ destruct H3. destruct H2.
+ intuition.
+ substs.
+ apply star_refl.
+ substs.
+ apply taured_val_id in H0.
+ simplify_eq H0; clear H0; intros; substs.
+ assumption.
+ simpl; auto.
+ exists x0 x1.
+ destruct H3. destruct H2.
+ intuition.
+ substs.
+ apply star_refl.
+ substs.
+ apply taured_val_id in H0.
+ simplify_eq H0; clear H0; intros; substs.
+ assumption.
+ simpl; auto.
+Qed.
+
+
+Inductive fork_comm_rel :  relation expr := 
+ | forkee_start : forall (e e' : livemodes), fork_comm_rel (E_apply (E_apply (E_constant CONST_fork) (E_live_expr (e))) (E_live_expr (e'))) (E_bind (E_apply (E_apply (E_constant CONST_fork) (E_live_expr (e'))) (E_live_expr (e))) (swapf))
+ | forkee_tau : forall  ( lm lm' : livemodes) (e : expr),  totalTauRed (E_bind ((E_live_expr lm')) (swapf)) (E_live_expr lm) /\  totalTauRed (E_bind ((E_live_expr lm')) (swapf)) e  -> fork_comm_rel (E_live_expr lm) e.
+
+
+Theorem fork_comm_wbsm : forall (p q : expr), fork_comm_rel p q -> ((forall (l : label) (p' : expr), labRed l p p' -> (exists (q' : expr), labRed l q q' /\ fork_comm_rel p' q') ) /\ (forall (l : label) (q' : expr), labRed l q q' -> (exists (p' : expr), labRed l p p' /\ fork_comm_rel p' q') )).
+Proof. 
+ intros.
+ splits.
+ induction H.
+ intros.
+ substs.
+ assert (L := H).
+ apply fork_lab_behave in H.
+ destruct H.
+ destruct H; destruct H.
+ substs.
+ assert (H0 := L).
+ apply fork_comm_labred in H0.
+ exists ((E_apply (E_apply (E_constant CONST_fork) (E_live_expr x0))
+          (E_live_expr x)) >>= swapf).
+ splits.
+ apply bind_lab_behave_front.
+ assumption.
+ apply forkee_start.
+ intuition.
+ destruct H0.
+ substs.
+ destruct H1.
+ destruct H.
+ destruct H.
+ destruct H.
+ destruct H.
+ assert (M:=H).
+ apply fork_comm_step_fin in H.
+ exists (E_live_expr x).
+ splits.
+ destruct H.
+ destruct H.
+ apply lab_r with (e1:= ((E_apply (E_apply (E_constant CONST_fork) (E_live_expr x1))
+      (E_live_expr x0)) >>= swapf))(e2:= ((E_live_expr x4) >>= swapf))(s:=x3).
+ splits.
+ assert (N:=H0).
+ apply fork_comm_taured in H0.
+ apply bind_tau_behave_front.
+ assumption.
+ apply JO_red_evalbind.
+ intuition.
+ elim H; intros.
+ apply tau_incl_totalTau in H2.
+ assumption.
+ apply fork_comm_taured in H0.
+ destruct H; destruct H; intuition.
+ apply forkee_tau with (lm':=x4).
+ splits.
+ assumption.
+ assumption.
+ intuition.
+ apply fork_comm_tau_fin in H1.
+ intuition.
+ destruct H2.
+ exists ( (E_live_expr x2) >>= swapf).
+ splits.
+ apply fork_comm_labred in H0.
+ inversion H0.
+ intuition.
+ substs.
+ apply lab_r with (e1:=(e1 >>= swapf))(e2:=(e2 >>= swapf))(s:=s).
+ splits.
+ apply bind_tau_behave_front.
+ assumption.
+ apply JO_red_evalbind.
+ assumption.
+ apply bind_tau_behave_front.
+ apply star_trans with (y:=(E_apply (E_apply (E_constant CONST_fork) (E_live_expr x1))
+          (E_live_expr x0))).
+ assumption.
+ assumption.
+ apply forkee_tau with (lm':=x2) .
+ splits.
+ intuition.
+ apply star_refl.
+ intros.
+ apply labred_not_val in H0.
+ simpl in H0; intuition.
+
+
+(* <- *)
+ 
+ inversion H.
+ substs.
+ intros.
+ apply fork_swap_lab_behave in H0.
+ intuition.
+ destruct H1; destruct H0; intuition; substs.
+ apply fork_comm_labred in H2.
+ exists (E_apply (E_apply (E_constant CONST_fork) (E_live_expr x0))
+          (E_live_expr x)).
+ splits.
+ assumption.
+ apply forkee_start.
+ destruct H1.
+ intuition.
+ apply fork_lab_behave in H1.
+ intuition.
+ destruct H0; destruct H0.
+ simplify_eq H0; clear H0; intros; substs.
+ destruct H1.
+ simplify_eq H0; clear H0; intros; substs.
+ destruct H3. destruct H0.
+ intuition.
+ destruct H0.
+ inversion H0.
+ substs.
+ exists (E_live_expr
+          (LM_expr
+             (
+                (E_taggingright
+                   (E_pair  (E_live_expr (LM_expr e0)) (E_constant CONST_unit)))))).
+ splits.
+ apply fork_comm_taured in H3.
+ apply lab_r with (e1:=(E_apply (E_apply (E_constant CONST_fork) (E_live_expr (LM_expr e0)))
+          (E_live_expr (LM_comp l))))(e2:=(E_live_expr
+     (LM_expr
+        (E_taggingright
+           (E_pair (E_live_expr (LM_expr e0)) (E_constant CONST_unit))))))(s:=x2).
+ splits.
+ assumption.
+ apply JO_red_forkdocomp2.
+ apply star_refl.
+ apply forkee_tau with (lm':=(LM_expr
+             (E_taggingleft
+                (E_taggingright
+                   (E_pair (E_constant CONST_unit) (E_live_expr (LM_expr e0))))))).
+ splits.
+ apply swapf_left_right_b.
+ simpl; auto.
+ simpl; auto.
+ assumption.
+ substs.
+
+
+ exists (E_live_expr
+          (LM_expr
+            (E_taggingleft
+             (E_taggingright
+                (E_pair (E_constant CONST_unit) (E_live_expr (LM_expr e0)) ))))).
+ splits.
+ apply fork_comm_taured in H3.
+ apply lab_r with (e1:=(E_apply (E_apply (E_constant CONST_fork) (E_live_expr (LM_comp l)))
+          (E_live_expr (LM_expr e0))))(e2:=(E_live_expr
+     (LM_expr
+        (E_taggingleft
+           (E_taggingright
+              (E_pair (E_constant CONST_unit) (E_live_expr (LM_expr e0))))))))(s:=x2).
+ splits.
+ assumption.
+ apply JO_red_forkdocomp1.
+ apply star_refl.
+ apply forkee_tau with (lm':=(LM_expr
+             (E_taggingright
+                (E_pair (E_live_expr (LM_expr e0)) (E_constant CONST_unit))))).
+ splits.
+ apply swapf_right_b.
+ simpl; auto.
+ simpl; auto.
+ assumption.
+ substs.
+ 
+ exists (E_live_expr
+          (LM_expr
+             (E_taggingleft
+                (E_taggingleft
+                   (E_pair (E_constant CONST_unit) (E_constant CONST_unit)))))).
+ splits.
+ apply fork_comm_taured in H3.
+ apply lab_r with (e1:=(E_apply (E_apply (E_constant CONST_fork) (E_live_expr (LM_comp l)))
+          (E_live_expr (LM_expr (E_constant CONST_unit)))))(e2:=(E_live_expr
+     (LM_expr
+        (E_taggingleft
+           (E_taggingleft
+              (E_pair (E_constant CONST_unit) (E_constant CONST_unit)))))))(s:=x2).
+ splits.
+ assumption.
+ apply JO_red_forkfincomp21.
+ apply star_refl.
+ apply forkee_tau with (lm':=(LM_expr
+             (E_taggingleft
+                (E_taggingleft
+                   (E_pair (E_constant CONST_unit) (E_constant CONST_unit)))))).
+ splits.
+ apply swapf_left_left_b.
+ simpl; auto.
+ simpl; auto.
+ assumption.
+ substs.
+
+ exists (E_live_expr
+          (LM_expr
+             (E_taggingleft
+                (E_taggingleft
+                   (E_pair (E_constant CONST_unit) (E_constant CONST_unit)))))).
+ splits.
+ apply fork_comm_taured in H3.
+ apply lab_r with (e1:=(E_apply
+          (E_apply (E_constant CONST_fork)
+             (E_live_expr (LM_expr (E_constant CONST_unit))))
+          (E_live_expr (LM_comp l))))(e2:=(E_live_expr
+     (LM_expr
+        (E_taggingleft
+           (E_taggingleft
+              (E_pair (E_constant CONST_unit) (E_constant CONST_unit)))))))(s:=x2).
+ splits.
+ assumption.
+ apply JO_red_forkfincomp12.
+ apply star_refl.
+ apply forkee_tau with (lm':=(LM_expr
+             (E_taggingleft
+                (E_taggingleft
+                   (E_pair (E_constant CONST_unit) (E_constant CONST_unit)))))).
+ splits.
+ apply swapf_left_left_b.
+ simpl; auto.
+ simpl; auto.
+ assumption.
+ substs.
+ induction x; induction x1.
+ apply fork_tau_behave_cc in H3.
+ discriminate H3.
+ apply fork_tau_behave_ce in H3.
+ discriminate H3.
+ apply fork_tau_behave_ec in H3.
+ discriminate H3.
+ assert (L:=H3).
+ substs.
+
+ apply fork_tau_behave_ee in H3.
+ intuition.
+ destruct H1. destruct H1; intuition.
+ discriminate H5.
+ destruct H3; destruct H1; intuition.
+ simplify_eq H6; clear H6; intros; substs.
+ exists (E_live_expr
+          (LM_expr (E_taggingleft (E_taggingright (E_pair  x1 (E_live_expr (LM_expr x))))))).
+ splits.
+ apply fork_comm_labred in H0.
+ apply fork_comm_taured_ee_laststep_h in L.
+ destruct L.
+ destruct H5.
+ destruct H5.
+ intuition.
+ simplify_eq  H6; clear H6; intros; substs.
+ simplify_eq  H5; clear H5; intros; substs.
+ destruct H8.
+ destruct H5.
+ intuition.
+ inversion H7.
+ substs.
+ inversion H5.
+ substs.
+ assert (E_apply (E_apply (E_constant CONST_fork) (E_live_expr (LM_expr x1)))
+       (E_live_expr (LM_expr x)) [s]--> [RL_tau]
+     E_live_expr
+       (LM_expr (E_taggingleft(E_taggingright (E_pair  x1 (E_live_expr (LM_expr x))))))).
+ apply JO_red_forkdeath1.
+ assumption.
+ apply fork_comm_taured in H6.
+ inversion H0; intuition.
+ substs.
+ apply lab_r with (e1:=e1)(e2:=e2)(s:=s0).
+ splits.
+ assumption.
+ assumption.
+ apply star_trans with (y:=(E_apply (E_apply (E_constant CONST_fork) (E_live_expr (LM_expr x0)))
+           (E_live_expr (LM_expr x2)))).
+ assumption.
+ apply star_trans with (y:=(E_apply (E_apply (E_constant CONST_fork) (E_live_expr (LM_expr x1)))
+          (E_live_expr (LM_expr x)))).
+ assumption.
+ apply S_star with (y:=(E_live_expr
+     (LM_expr
+        (E_taggingleft (E_taggingright (E_pair x1 (E_live_expr (LM_expr x)))))))).
+ apply tStep with (s:=s).
+ assumption.
+ apply star_refl.
+ exists expr0 expr5 (LM_expr (E_taggingright (E_pair (E_live_expr (LM_expr x)) x1))).
+ splits; [reflexivity | reflexivity ].
+ 
+ apply forkee_tau with (lm':=(LM_expr (E_taggingright (E_pair (E_live_expr (LM_expr x)) x1)))).
+  splits.
+ apply swapf_right_b.
+ simpl; auto.
+ assumption.
+ assumption.
+
+ destruct H1. destruct H1; intuition.
+ simplify_eq H7; clear H7; intros; substs.
+ exists (E_live_expr (LM_expr (E_taggingleft (E_taggingleft (E_pair x1 x)))) ).
+ splits.
+ apply fork_comm_labred in H0.
+ inversion H0.
+ substs.
+ apply lab_r with (e1:=e1)(e2:=e2)(s:=s).
+ splits.
+ intuition.
+ intuition.
+ intuition.
+ apply star_trans with (y:=(E_apply
+          (E_apply (E_constant CONST_fork) (E_live_expr (LM_expr expr0)))
+          (E_live_expr (LM_expr expr5)))).
+ 
+ assumption.
+
+ apply fork_comm_taured_ee_laststep_h in L.
+ destruct L.
+ destruct H8.
+ destruct H8.
+ intuition.
+ simplify_eq  H10; clear H10; intros; substs.
+ simplify_eq  H8; clear H8; intros; substs.
+ destruct H12.
+ destruct H8.
+ intuition.
+ inversion H11.
+ substs.
+ inversion H8.
+ substs.
+ assert (E_apply (E_apply (E_constant CONST_fork) (E_live_expr (LM_expr x1)))
+       (E_live_expr (LM_expr x)) [s0]--> [RL_tau]
+     E_live_expr (LM_expr (E_taggingleft (E_taggingleft (E_pair x1 x))))).
+ apply JO_red_forkdeath12.
+ assumption.
+ assumption.
+ apply fork_comm_taured in H10.
+ apply star_trans with (y:=(E_apply (E_apply (E_constant CONST_fork) (E_live_expr (LM_expr x1)))
+          (E_live_expr (LM_expr x)))).
+ assumption.
+ apply S_star with (y:=(E_live_expr (LM_expr (E_taggingleft (E_taggingleft (E_pair x1 x)))))).
+ apply tStep with (s:=s0).
+ assumption.
+ apply star_refl.
+ exists expr0 expr5 (LM_expr (E_taggingleft (E_taggingleft (E_pair x x1)))).
+ splits; [reflexivity | reflexivity ].
+ 
+ apply forkee_tau with (lm':=(LM_expr (E_taggingleft (E_taggingleft (E_pair x x1))))).
+  splits.
+ apply swapf_left_left_b.
+ simpl; auto.
+ assumption.
+ assumption.
+
+ destruct H1. destruct H1; intuition.
+ simplify_eq H6; clear H6; intros; substs.
+ exists (E_live_expr
+          (LM_expr
+             (
+                (E_taggingright (E_pair (E_live_expr (LM_expr x1)) x ))))).
+ splits.
+ apply fork_comm_labred in H0.
+  inversion H0.
+ substs.
+ apply lab_r with (e1:=e1)(e2:=e2)(s:=s).
+ splits.
+ intuition.
+ intuition.
+ intuition.
+ apply star_trans with (y:=(E_apply
+          (E_apply (E_constant CONST_fork) (E_live_expr (LM_expr expr0)))
+          (E_live_expr (LM_expr expr5)))).
+ 
+ assumption.
+ 
+ apply fork_comm_taured_ee_laststep_h in L.
+ destruct L.
+ destruct H7.
+ destruct H7.
+ intuition.
+ simplify_eq  H9; clear H9; intros; substs.
+ simplify_eq  H7; clear H7; intros; substs.
+ destruct H11.
+ destruct H7.
+ intuition.
+ inversion H10.
+ substs.
+ inversion H7.
+ substs.
+ assert (E_apply (E_apply (E_constant CONST_fork) (E_live_expr (LM_expr x1)))
+       (E_live_expr (LM_expr x)) [s0]--> [RL_tau]
+     E_live_expr
+       (LM_expr
+          (
+             (E_taggingright (E_pair (E_live_expr (LM_expr x1)) x))))).
+ apply JO_red_forkdeath2.
+ assumption.
+ apply fork_comm_taured in H9.
+ apply star_trans with (y:=(E_apply (E_apply (E_constant CONST_fork) (E_live_expr (LM_expr x1)))
+          (E_live_expr (LM_expr x)))).
+ assumption.
+ apply S_star with (y:=(E_live_expr
+     (LM_expr (E_taggingright (E_pair (E_live_expr (LM_expr x1)) x))))).
+ apply tStep with (s:=s0).
+ assumption.
+ apply star_refl.
+ exists expr0 expr5 (LM_expr
+     (E_taggingleft (E_taggingright (E_pair x (E_live_expr (LM_expr x1)))))).
+ splits; [reflexivity | reflexivity ].
+ 
+ apply forkee_tau with (lm':=(LM_expr
+             (E_taggingleft
+                (E_taggingright (E_pair x (E_live_expr (LM_expr x1))))))).
+  splits.
+ apply swapf_left_right_b.
+ simpl; auto.
+ simpl; auto.
+ assumption.
+ 
+ intros.
+ substs.
+ intuition.
+ assert (totalTauRed (E_live_expr lm' >>= swapf) (E_live_expr lm) /\ tauRed (E_live_expr lm' >>= swapf) q).
+ splits.
+ assumption.
+ apply tau_incl_totalTau.
+ assumption.
+
+ apply ttau_prefix in H0.
+ intuition.
+ inversion H3.
+
+ intuition; substs.
+ assert (~ (labRed l q q')).
+ apply ttr_val_not_labred with (v:= (E_live_expr lm)).
+ intuition.
+ simpl.
+ auto.
+ contradiction.
+ apply taured_val_id in H4; substs.
+ apply labred_not_val in H3.
+ simpl in H3; intuition.
+ simpl; auto.
+
+ Qed.
